- Consider the same slight variation on the 2D Model Problem, T(a,b), defined in last week's homework.
    
    - Is there an ordering of the equations and unknowns for which SOR(w) converges, for T(a,b), for some values of w? What ordering, and which values of w?
In HW12, we showed that $T(a,b)$ is symmetric positive definite. Theorem 12.4 states that 
![[Pasted image 20231201161727.png|700]]
and such SOR converges for $0<w<2$ for any ordering.

<div style="page-break-after: always;"></div>

```ad-question
title: 6.15 Part 1
Confirm that 
$$T^{(i-1)}=4 \cdot P_{i}^{i-1}T^{(i)}P_{i-1}^{i}=8\cdot P_{i}^{i-1}T^{(i)}(P_{i}^{i-1})^{T}$$

```

We have that
$$P_{i}^{i-1}=\begin{bmatrix}1/4 & 1/2 & 1/4 \\   &     & 1/4 & 1/2  & 1/4 \\  &   & & \ddots  & \ddots  & \ddots  \\  &    &   &   & & 1/4 & 1/2 & 1/4\end{bmatrix}, \qquad P_{i-1}^{i}=\begin{bmatrix}1/2 \\ 1 \\ 1/2  & 1/2 \\  & 1 & \ddots  \\  & 1/2 & \ddots  & 1/2 \\  &   & \ddots  & 1 \\  &   &   &  1/2\end{bmatrix}.$$
Let's compute the matrix multiplications,
$$\begin{align*}
4P^{i-1}_{i}T^{(i)}P_{i-1}^{i}&= \begin{bmatrix}1/2 & 1 & 1/2 \\   &     & 1/2 & 1  & 1/2 \\  &   & & \ddots  & \ddots  & \ddots  \\  &    &   &   & & 1/2 & 1 & 1/2\end{bmatrix}\begin{bmatrix} 2 & -1\\
-1 & 2 & -1\\
 & \ddots  & \ddots  & \ddots \\
 &   &   -1 & 2 \end{bmatrix} \begin{bmatrix}1 \\ 2 \\ 1  & 1 \\  & 2 & \ddots  \\  & 1 & \ddots  & 1 \\  &   & \ddots  & 2 \\  &   &   &  1\end{bmatrix}\\
&= \begin{bmatrix}1/2 & 1 & 1/2 \\   &     & 1/2 & 1  & 1/2 \\  &   & & \ddots  & \ddots  & \ddots  \\  &    &   &   & & 1/2 & 1 & 1/2\end{bmatrix}\begin{bmatrix}0 & \dots  & \dots  & 0\\
2 & -1\\
0 & \dots & \dots  & 0 \\
-1 & 2 & -1\\
0 & \dots & \dots  & 0 \\
0 & -1 & 2 & -1\\
\vdots  & \vdots  & \vdots  & \vdots \\
0 & 0 & -1 & 2\\
0 & \dots  & \dots  & 0\end{bmatrix}
\end{align*}$$
where in the last matrix we have an alternating pattern between zero rows and rows with $-1,2,-1$. This arises since row number $j$ in the resulting matrix is $2 \cdot$ row $j$ - row $j-1$ - row $j+1$ in $P_{i-1}^{i}$.

Finally, we see that 
$$\begin{bmatrix}1/2 & 1 & 1/2 \\   &     & 1/2 & 1  & 1/2 \\  &   & & \ddots  & \ddots  & \ddots  \\  &    &   &   & & 1/2 & 1 & 1/2\end{bmatrix}\begin{bmatrix}0 & \dots  & \dots  & 0\\
2 & -1\\
0 & \dots & \dots  & 0 \\
-1 & 2 & -1\\
0 & \dots & \dots  & 0 \\
0 & -1 & 2 & -1\\
\vdots  & \vdots  & \vdots  & \vdots \\
0 & 0 & -1 & 2\\
0 & \dots  & \dots  & 0\end{bmatrix}=\begin{bmatrix} 2 & -1\\
-1 & 2 & -1\\
 & \ddots  & \ddots  & \ddots \\
 &   &   -1 & 2 \end{bmatrix}=T^{(i-1)}$$
 since we are again taking a weighted average of the rows, but now row number $j$ is comprised of row $2j$ - row $2j-1$ - row $2j+1$ in the second matrix. Since rows $2j\pm1$ are zero rows, we only take row $2j$.

Note that $P_{i-1}^{i}=2(P_{i}^{i-1})^{T}$, then we get the last equality and what we wanted to show,
$$T^{(i-1)}=4P^{i-1}_{i}T^{(i)}P_{i-1}^{i}=4P^{i-1}_{i}T^{(i)}2(P_{i}^{i-1})^{T}=8P^{i-1}_{i}T^{(i)}(P_{i}^{i-1})^{T}$$

```ad-question
title: 6.15 Part 2
Confirm that $Z^{(i-1)}PZ^{(i)}=\Lambda _{P}$, where $\Lambda _{P}$ is nearly diagonal:
$$\lambda _{P,jk}=\begin{cases}
(+1+\text{cos}\frac{\pi j }{2^{i}})/\sqrt{8} & \quad\text{for }k=j \\
(-1+\text{cos}\frac{\pi  j}{2^{i}})/\sqrt{8} & \quad\text{for }k=2^{i}-j \\
0 &  \quad\text{else}
\end{cases}$$

```
We have that $T^{(i)}=Z^{(i)}\Lambda Z^{(i)}$,
$$\begin{align*}
T^{(i-1)}&= 8 PT^{(i)}P^{T}\\
Z^{(i-1)} \Lambda ^{(i-1)}Z^{(i-1)}&= 8PZ^{(i)}\Lambda ^{(i)}Z^{(i )}P^{T}\\
\Lambda ^{(i-1)}&= 8Z^{(i-1)}PZ^{(i)}\Lambda ^{(i)}(Z^{(i-1)}PZ^{(i)})^{T}\\
\Lambda _{P}\Lambda ^{(i)}\Lambda _{P}^{T}&= \Lambda ^{(i-1)}/8
\end{align*}$$
Looking at index $jk$,
$$\sum_{l}^{}\lambda _{P,jl} \lambda _{P,kl} \cdot \lambda^{(i)} _{l}=\begin{cases}
\lambda ^{(i-1)}_{j}/8 & \quad\text{for }j=k \\
0 & \quad\text{else}
\end{cases}$$
So we get the two equations 
$$\begin{align*}
\sum_{l}^{}\lambda _{P,kl}^{2}\cdot \lambda _{l} ^{(i)}&= \lambda _{k}^{(i-1)}/8\\
	\sum_{l}^{}\lambda _{P,kl}\cdot \lambda _{P,jl}\cdot \lambda _{l}^{(i)}&= 0
\end{align*}$$
which I will verify seperately.
Let's verify the first equation,
$$\lambda _{P,kk}^{2}\cdot \lambda _{k}^{(i)}+\lambda _{P,k,2^{i}-k}^{2}\cdot \lambda _{2^{i}-k}^{(i)}=\lambda _{k}^{(i-1)}/8$$
substituting in for the different $\lambda$'s, (using the eigenvalues of $T_{N}$ from HW11)
$$\left(1+\text{cos}\frac{\pi k}{2^{i}}\right)^{2}\cdot 2 \left(1- \text{cos}\frac{\pi k}{2^{i}} \right)+\left(-1+\text{cos}\frac{\pi k}{2^{i}}\right)^{2}\cdot 2\left(1-\text{cos}\frac{\pi (2^{i}-k)}{2^{i}} \right)=2\left(1-\text{cos}\frac{\pi k}{2^{i-1}}\right)$$
Notice that $\text{cos}\frac{\pi (2^{i}-k)}{2^{i}}=\text{cos}\left(\pi - \frac{\pi k}{2^{i}}\right)=-\text{cos}\frac{\pi k}{2^{i}}$. For simplicities sake, denote $c=\text{cos}\frac{\pi k}{2^{i}}$, and our equation becomes
$$\begin{align*}
(1+c)^{2}(1-c)+(-1+c)^{2}(1+c)&= 1-\text{cos}\frac{\pi k}{2^{i-1}}\\
(1+2c+c^{2})(1-c)+(1-2c+c^{2})(1+c)&= 1-\text{cos}\frac{\pi k}{2^{i-1}}\\
1-c+2c-2c^{2}+c^{2}-c^{3}+1+c-2c-2c^{2}+c^{2}+c^{3}&= 1-\text{cos}\frac{\pi k}{2^{i-1}}\\
2-2c^{2}&= 1-\text{cos}\frac{\pi k}{2^{i-1}}\\
2 \left(1-\text{cos}^{2}\frac{\pi k}{2^{i}} \right) &= 1-\text{cos}\frac{\pi k}{2^{i-1}}\\
\text{cos}^{2}\frac{\pi k}{2^{i}}&= \frac{1+\text{cos}\left(2\cdot \frac{\pi k}{2^{i}} \right)}{2}
\end{align*}$$
which is a trig identity. $\Lambda _{P}$ satisfies the first equation. 

Moving on to the second equation,
$$\sum_{l}^{}\lambda _{P,kl}\cdot \lambda _{P,jl}\cdot \lambda _{l}^{(i)}= 0 $$
We know that $j≠k$. If also $j≠2^{i}-k$, then all of the summands are zero.
Assuming that $j=2^{i}-k$, then the only nonzero summands are when $l=j$ and when $l=k$. Writing these out,
$$\lambda _{P,kj}\cdot \lambda _{P,jj}\cdot \lambda _{j}^{(i)}+\lambda _{P,kk}\cdot \lambda _{P,jk}\cdot \lambda _{k}^{(i)}$$
Letting $j=2^{i}-k$, we get

$$\begin{align*}
&\quad \lambda _{P,k,2^{i}-k}\cdot \lambda _{P,2^{i}-k,2^{i}-k}\cdot \lambda _{2^{i}-k}^{(i)}+\lambda _{P,kk}\cdot \lambda _{P,2^{i}-k,k}\cdot \lambda _{k}^{(i)}\\
&= \left(-1+\text{cos}\frac{\pi k}{2^{i}}\right)\cdot \left(1+\text{cos}\frac{\pi (2^{i}-k)}{2^{i}}\right)\cdot 2\left(1-\text{cos}\frac{\pi (2^{i}-k)}{2^{i}} \right)\\
&\quad +\left(1+\text{cos}\frac{\pi k}{2^{i}}\right)\left(-1+\text{cos}\frac{\pi (2^{i}-k)}{2^{i}} \right)\cdot 2\left(1-\text{cos}\frac{\pi k}{2^{i}}\right)\\
&= \left(-1+\text{cos}\frac{\pi k}{2^{i}}\right)\cdot \left(1-\text{cos}\frac{\pi k}{2^{i}}\right)\cdot 2\left(1+\text{cos}\frac{\pi k}{2^{i}} \right)\\
&\quad +\left(1+\text{cos}\frac{\pi k}{2^{i}}\right)\left(-1-\text{cos}\frac{\pi k}{2^{i}} \right)\cdot 2\left(1-\text{cos}\frac{\pi k}{2^{i}}\right)\\
&= 2(-1+c)(1-c)(1+c)+2(1+c)(1-c)(1-c)\\
&= 2(1-c)(1+c)(-1+c+1-c)\\
&= 0
\end{align*}$$
and such $\Lambda _{P}$ as defined satisfies the second equation as well.


