![[Pasted image 20241207112902.png|800]]
$$
\begin{bmatrix}
 & D & a & T & \mu & k_{B} \\
m  & 2 & 1 & 0 & -1 & 2\\
s  & -1 & 0 & 0 & -1 & -2\\
kg  & 0 & 0 & 0 & 1 & 1\\
K & 0 & 0 & 1 & 0 & -1
\end{bmatrix}
$$
We see clearly that $a,T,\mu,k_{B}$ are dimensionally independant and we can therefore choose them as the core variables.
$$
\begin{align}
\mu & = kgm^{-1}s^{-1} \\
\frac{\mu}{k_{B}} & =\frac{kgm^{-1}s^{-1}}{kgm^{2}s ^{-2}K^{-1}}=m^{-3}sK \\
\frac{\mu}{k_{B}T} & =m^{-3}s \\
\frac{\mu D}{k_{B}T} & =m^{-3}s\cdot m^{2}s^{-1}=m^{-1} \\
\pi=\frac{\mu Da}{k_{B}T} & =1
\end{align}
$$
So there exists a function such that
$$
f(\pi,a,T,\mu,k_{B})=0
$$
since we could choose different units for the different variables, this implies that
$$
f(\pi)=0\implies \pi=C
$$
Then,
$$
D=C \cdot \frac{k_{B}T}{\mu a}
$$



![[Pasted image 20241207112911.png|800]]

Setting the derivatives to zero gives that $v=-u-1=-(u+1)$ and
$$
\begin{align}
u^3+4u^2-\underbrace{ (u+1)^{3} }_{ (u+1)(u^2+2u+1) }-u-1-3 & =0 \\
4u^2-2u^2-u-u^2-2u-1-u-1-3 & =0 \\
u^2-4u-5 & =0 \\
(u-5)(u+1) & =0
\end{align}
$$
Giving us the equilibrium points
$$
(u,v)=(5,-6) \cup(-1,0)
$$

The jacobian is
$$
J(u,v)=\begin{bmatrix}
3u^2+8u & 3v^2+1 \\
1 & 1
\end{bmatrix}
$$
$$
\begin{align}
J(5,-6) & =\begin{bmatrix}
115 & 109 \\
1 & 1
\end{bmatrix} \\
J(-1,0) & =\begin{bmatrix}
-5 & 1 \\
1 & 1
\end{bmatrix}
\end{align}
$$
See that $\det J(5,-6)=115-109=6>0$ and $\mathrm{Tr}=116>0$ which means that $(5,-6)$ is unstable. 
$\det J(-1,0)=-5-1=-6<0$ so $(-1,0)$ is also unstable.


![[Pasted image 20241207112923.png|800]]
$$
\begin{align}
\frac{ \partial u }{ \partial t } +PDP^{-1}\frac{ \partial u }{ \partial x }  & =0 \\
P^{-1}\frac{ \partial u }{ \partial t } +DP^{-1}\frac{ \partial u }{ \partial x }  & =0 \\
\frac{ \partial v }{ \partial t } +D\frac{ \partial v }{ \partial x }  & =0 \\
\frac{ \partial v_{1} }{ \partial t } +2\frac{ \partial v_{1} }{ \partial x }  & =0 \\
\frac{ \partial v_{2} }{ \partial t } +4\frac{ \partial v_{2} }{ \partial x }  & =0
\end{align}
$$
the initial values can be found as
$$
\begin{bmatrix}
v_{1}^0 \\
v_{2}^0 
\end{bmatrix}=\begin{bmatrix}
\frac{1}{2} & -\frac{1}{2} \\
\frac{1}{2} & \frac{1}{2}
\end{bmatrix}\begin{bmatrix}
x^2 \\
2x
\end{bmatrix}=\begin{bmatrix}
\frac{x^2}{2}-x \\
\frac{x^2}{2}+x
\end{bmatrix}
$$


First $v_{1}$, then $x(t)=2t+x_{0}$ such that $x_{0}=x-2t$. Then,
$$
\begin{align}
v_{1}(x,t) & =v_{1}^0(x-2t)=\frac{1}{2}(x-2t)^2-x+2t  \\
v_{2}(x,t) & =v_{2}^0(x-4t)=\frac{1}{2}(x-4t)^2+x-4t \\
v(x,t) & =\begin{bmatrix}
\frac{x^2}{2}-2xt+2t^2-x+2t \\
\frac{x^2}{2}-4xt+8t^2+x-4t
\end{bmatrix}
\end{align}
$$

$$
\begin{align}
u(x,t) & =Pv(x,t) \\
 & =\begin{bmatrix}
1 & 1 \\
-1 & 1
\end{bmatrix}\begin{bmatrix}
\frac{x^2}{2}-2xt+2t^2-x+2t \\
\frac{x^2}{2}-4xt+8t^2+x-4t
\end{bmatrix} \\
 & =\begin{bmatrix}
x^2-6xt+10t^2-2t \\
-2xt+6t^2+2x-6t
\end{bmatrix}
\end{align}
$$



![[Pasted image 20241207112928.png|800]]
$$
x(t)=(2u_{0}(x_{0})-1)t+x_{0}
$$
when $x_{0}<0$, $x(t)=x_{0}-t$
when $x_{0}>0$, $x(t)=(2a-1)t+x_{0}$

![[IMG_10C8E60C5869-1.jpeg|500]]
We get a rarefaction wave between $x=-t$ and $x=(2a-1)t$.

The solution in the rarefaction wave is given by
$$
u(x,t)=f^{-1}\left( \frac{x}{t} \right)
$$
We have $f(u)=2u-1\implies f^{-1}(u)=\frac{u+1}{2}$. So when $-t<x<(2a-1)t$, the solution is
$$
\begin{align}
u(x,t)=\frac{\left( \frac{x}{t}+1 \right)}{2}=\frac{x}{2t}+\frac{1}{2}
\end{align}
$$
the full solution is
$$
u(x,t)=\begin{cases}
0 & x<-t \\
\frac{x}{2t}+\frac{1}{2} & -t<x<(2a-1)t \\
a & (2a-1)t<x
\end{cases}
$$
When $a<0$, we have a shock
![[Pasted image 20241207130746.png|500]]

When we have a shock, we need to determine it speed by setting $F(u)=\int f(u)\text{ d}u$ and
$$
V= \frac{F(u^-)-F(u^+)}{u^--u^+}
$$
The position of the shock is then $s(t)=Vt+x_{s}$ where $x_{s}$ is the starting position of the shock. The solution is then given by
$$
u(x,t)=\begin{cases}
u^- & x<s(t) \\
u^+ & x>s(t)
\end{cases}
$$

In our case, $F(u)=u^2-u$ so the speed is
$$
V= \frac{0-(a^2-a)}{0-a}=a-1
$$
The position of the shock is $s(t)=(a-1)t$ so the solution is
$$
u(x,t)=\begin{cases}
0 & x<(a-1)t \\
a & x>(a-1)t
\end{cases}
$$



![[Pasted image 20241207112933.png|800]]
$$
u_{t}+(2u-1)u_{x}=0
$$
The characteristics are $x(t)=x_{0}-t$ for $x_{0}<0$
$x(t)=x_{0}+(2bx_{0}-1)t$ for $0<x_{0}<1$
$x(t)=x_{0}+(2b-1)t$ for $x_{0}>1$.

![[Pasted image 20241207133823.png|500]]
$$
u(x,t)=u_{0}(x_{0}(x,t))
$$
for $0<x_{0}<1$
$$
\begin{align}
x & =x_{0}+2bx_{0}t-t \\
(2bt+1)x_{0} & =x+t \\
x_{0} & =\frac{x+t}{2bt+1} \\
u_{0}(x_{0}) & =bx_{0}
\end{align}
$$
$$
u(x,t)=\begin{cases}
0 & x<-t \\
b \frac{x+t}{2bt+1}  & -t<x<(2b-1)t+1 \\
b & (2b-1)t+1<x
\end{cases}
$$

![[Pasted image 20241207112938.png|800]]
### Outer solution
To find the outer solution, we let $\epsilon\to0$ so 
$$
\begin{align}
4y'+(\sin x)y^{2} & =0 \\
y^{-2} \frac{\text{d}y}{\text{d}x}  & =-\frac{1}{4}\sin x \\
\int y^{-2}\text{ d} y & =\int-\frac{1}{4}\sin x\text{ d} x \\
-y^{-1} & =-\frac{1}{4}\cos x+C \\
y (x)& =\frac{1}{ \frac{1}{4}\cos x+C}=\frac{4}{\cos x+C} \\
y(\pi) & = \frac{4}{-1+C}=1 \\
C & =5 \\
y(x) & =\frac{4}{\cos x+5}
\end{align}
$$
### Inner solution
Let $\eta=\frac{\epsilon}{\delta(\epsilon)}$ and postulate that
$$
Y\left( \frac{x}{\delta(\epsilon)} \right)=y(x)
$$
Then the equation for $Y$ is
$$
\begin{align}
\frac{\epsilon}{\delta(\epsilon)^2}Y''+\frac{4}{\delta(\epsilon)}Y'+(\sin x)Y^2 & =0 \\
\frac{\epsilon}{\delta(\epsilon)}Y''+4Y'+\delta(\epsilon)(\sin x)Y^2  & =0 \\
\text{let }\delta(\epsilon)=\epsilon\implies \qquad Y''+4Y'+\epsilon(\sin x)Y^2 & =0 \\
\text{let }\epsilon\to0\qquad Y''+4Y' & =0
\end{align}
$$
This can be solved as
$$
\begin{align}
\lambda^2+4\lambda & =0 \\
\lambda_{1} & =0 \\
\lambda_{2} & =-4
\end{align}
$$
which gives the general solution
$$
\begin{align}
Y(\eta ) & =C_{1}e^{ \lambda_{1}\eta }+C_{2}e^{ \lambda_{2}\eta } \\
 & =C_{1}+C_{2}e^{ -4\eta } \\
Y(0) & =C_{1}+C_{2}=0 \\
Y(\eta) & =C_{1}(1-e^{ -4\eta })
\end{align}
$$
Matching condition:
$$
\begin{align}
\lim_{ x \to 0 } y(x) & =\lim_{ \eta \to \infty } Y(\eta) \\
\frac{4}{\cos0+5} & =C_{1} \\
\frac{2}{3} & =C_{1} \\
Y(\eta) & =\frac{2}{3}(1-e^{ -4\eta })
\end{align}
$$
The uniform solution is then
$$
\begin{align}
y^{u}(x) & =y(x)+Y\left( \frac{x}{\epsilon} \right)-\lim_{ x \to 0 } y(x) \\
 & =\frac{4}{\cos x+5}+\frac{2}{3}(1-e^{ -4x/\epsilon })-\frac{2}{3} \\
 & =\frac{4}{\cos x+5}-\frac{2}{3}e^{ -4x/\epsilon }
\end{align}
$$


![[Pasted image 20241207112948.png|800]]
Assume that the rate at which sick people infect healthy people are $\alpha$, and that the rate of recovery is $\beta$. Then the change in sick people are
$$
\frac{ \partial u }{ \partial t } =\alpha uv-\beta u
$$
since the amount of new infections rely on both the amount of sick and amount of healthy, while the rate of recovery only relies on the amount of sick people. Since $v(t)=N-u(t)$, we can rewrite this as
$$
\frac{ \partial u }{ \partial t }=\alpha u(N-u)-\beta u
$$
Letting $u\to Nu$ and $t\to Tt$,
$$
\begin{align}
\frac{N}{T}\frac{ \partial u }{ \partial t }  & =\alpha Nu(N-Nu)-\beta Nu \\
\frac{ \partial u }{ \partial t }  & =\alpha NTu(1-u)-\beta Tu
\end{align}
$$
Letting $T=\frac{1}{\beta}$,
$$
\begin{align}
\frac{ \partial u }{ \partial t }  & =\frac{\alpha N}{\beta}u(1-u)-u \\
\frac{ \partial u }{ \partial t }  & =\mu u(1-u)-u
\end{align}
$$
Denote
$$
\frac{ \partial u }{ \partial t } =f(u,\mu)=\mu u(1-u)-u
$$
$\mu=\frac{\alpha}{\beta}N$
We will always have the equilibrium point $u=0$, where the derivative is $\frac{ \partial f }{ \partial u }=\mu-1$.  So this equilibrium point is stable if $\mu<1$.
We can find another equilibrium point where $u>0$:
$$
\begin{align}
\mu(1-u)-1 & =0 \\
u & =\frac{\mu-1}{\mu}
\end{align}
$$

We can rewrite $f(u, \mu)=0$ to
$$
u(1-u)=\frac{u}{\mu}
$$
![[Pasted image 20241207163429.png|500]]
We see that there is a second equilibrium point at $u=\frac{\mu-1}{\mu}$, but only if $\mu$ is large enough. If the derivatives at the origo fulfill
$$
\begin{align}
1-2u< \frac{1}{\mu} \\
\mu<1
\end{align}
$$
then there is no second equilibrium point. 

This second equilibrium point is stable if 
$$
\begin{align}
\frac{ \partial f }{ \partial u } \left( \frac{\mu-1}{\mu} \right) & <0 \\
\mu\left( 1-2 \frac{\mu-1}{\mu} \right)-1 & <0 \\
\mu-2\mu+2-1 & <0 \\
1 & <\mu
\end{align}
$$
so if the equilibrium point exist, then it is stable.

![[Pasted image 20241207164637.png|800]]
![[Pasted image 20241207164647.png|800]]
![[Pasted image 20241207164628.png|800]]

For gas:

$$
\begin{align}
\frac{\text{d}}{\text{d}t} \rho_{g}\phi A \int_{a}^bS(x,t)\text{ d} x & =\rho_{g}q_{g}(a,t)A-\rho_{g}q_{g}(b,t)A \\
\frac{\text{d}}{\text{d}t} \rho_{g}\phi A \int_{a}^bS(x,t)\text{ d} x & =\rho_{g}A\int_{a}^b-\frac{ \partial q_{g}(x,t) }{ \partial x } \text{ d} x \\
\phi \frac{\text{d}S(x,t)}{\text{d}t}  & =-\frac{ \partial q_{g}(x,t) }{ \partial x } 
\end{align}
$$
For water:
$$
\begin{align}
\frac{\text{d}}{\text{d}t} \rho_{w}\phi A \int_{a}^b(1-S(x,t))\text{ d} x & =\rho_{w}q_{w}(a,t)A-\rho_{w}q_{w}(b,t)A \\
\frac{\text{d}}{\text{d}t} \rho_{w}\phi A \int_{a}^b(1-S(x,t))\text{ d} x & =\rho_{w}A\int_{a}^b-\frac{ \partial q_{w}(x,t) }{ \partial x } \text{ d} x \\
-\phi \frac{\text{d}S(x,t)}{\text{d}t}  & =-\frac{ \partial q_{w}(x,t) }{ \partial x } 
\end{align}
$$
Adding the two equations together, we get
$$
0=-\frac{ \partial q_{g} }{ \partial x } -\frac{ \partial q_{w} }{ \partial x } =-\frac{ \partial q }{ \partial x } 
$$
and hence this quantity does not depend on $x$.

$$
\begin{align}
q_{w}+q_{g} & =-\frac{k}{\mu_{g}}S\frac{ \partial p }{ \partial x } -\frac{k}{\mu_{w}}(1-S)\frac{ \partial p }{ \partial x }  \\
 & =-k\frac{ \partial p }{ \partial x }  \left( \frac{S}{\mu_{g}}+\frac{1-S}{\mu_{w}} \right) \\
 q(t)& =-k \frac{ \partial p }{ \partial x } \lambda_{T}(S) \\
\frac{q(t)}{\lambda_{T}(S)} & =-k 
\end{align}
$$