![[Pasted image 20241208131647.png|800]]
$E=\frac{1}{2}mv^2=kgm^2s^{-2}$
$$
\begin{bmatrix}
 & E & L & A & \rho & T \\
m & 2 & 1 & 1 & -1 & 1 \\
kg & 1 & 0 & 0 & 1 & 1 \\
s & -2 & 0 & 0 & 0 & -2
\end{bmatrix}
$$
We see that $A$, $\rho$ and $T$ are dimensionally independant since there is no $\alpha$, $\beta$, $\gamma$ such that
$$
[A^\alpha\rho^\beta T^\gamma]=1
$$
and the detereminant of the matrix
$$
\det\begin{bmatrix}
1 & -1 & 1 \\
0 & 1 & 1 \\
0 & 0 & -2
\end{bmatrix}=-2\neq0
$$
$$
\begin{align}
E & =kgm^{2}s^{-2} \\
\frac{E}{T} & =m \\
\pi_{1}=\frac{E}{TA} & =1
\end{align}
$$
There is another dimensionless variable that can be found as
$$
\begin{align}
\pi_{2}=\frac{L}{A}
\end{align}
$$


So there must exists a function such that $g(\pi_{1},\pi_{2},A,\rho,T)=0$, and since we can choose any units for $A$, $\rho$, and $T$, 
$$
g(\pi_{1},\pi_{2})=0\implies \pi_{1}=f(\pi_{2})
$$
Then
$$
\begin{align}
\frac{E}{TA} & =f\left( \frac{L}{A} \right) \\
E & =TAf\left( \frac{L}{A} \right)
\end{align}
$$
![[Pasted image 20241208133543.png|800]]
$$
\begin{align}
\underbrace{ E }_{ kgm^2s^{-2} } & =\hbar \underbrace{ \omega }_{ s^{-1} }&\implies[\hbar]=kgm^2s^{-1} \\
\underbrace{ F }_{ kgms^{-2} } & =G  \underbrace{ \frac{m_{1}m_{2}}{r^2} }_{ kg^2m^{-2} }&\implies[G]=kg^{-1}m^3s^{-2} \\
\underbrace{ E }_{ kgm^2s^{-2} } & =\underbrace{ m }_{ kg }c^2&\implies[c]=ms^{-1}
\end{align}
$$

$$
\begin{align}
\hbar & =val(\hbar)ML^2T^{-1} =1\cdot \tilde{M}\tilde{L}^2\tilde{T}^{-1}\\
G & =val(G)M^{-1}L^3T^{-2} =1\cdot \tilde{M}^{-1}\tilde{L}^3\tilde{T}^{-2}\\
c & =val(c)LT^{-1}=1\cdot \tilde{L}\tilde{T}^{-1}
\end{align}
$$

$$
\begin{align}
L & =cT \\
\hbar & =Mc^2T^2T^{-1}\implies M=\frac{\hbar}{c^2T} \\
G & =\left( \frac{\hbar}{c^2T} \right)^{-1}c^3T^3T^{-2}=\frac{c^5T^2}{\hbar} \\
T & =\sqrt{ \frac{G\hbar}{c^5} } \\
L & =\sqrt{ \frac{G\hbar}{c^3} } \\
M & =\frac{\hbar}{c^2}\sqrt{ \frac{c^5}{G\hbar} }=\sqrt{ \frac{ch}{G} }
\end{align}
$$


![[Pasted image 20241208141712.png|800]]
$$
\begin{align}
u_{1}+u_{2} & =0 \\
-k\lambda_{1}(S)\left( \frac{ \partial p }{ \partial x } +\rho_{1}g\sin\alpha \right)-k\lambda_{2}(S)\left( \frac{ \partial p }{ \partial x } +\rho_{2}g\sin\alpha \right) & =0 \\
-k(\lambda_{1}(S)+\lambda_{2}(S))\frac{ \partial p }{ \partial x } -kg\sin\alpha(\rho_{1}\lambda_{1}(S)+\rho_{2}\lambda_{2}(S)) & =0 
\end{align}
$$
$$
\begin{align}
\frac{ \partial p }{ \partial x }  & =-g\sin\alpha \frac{\rho_{1}\lambda_{1}(S)+\rho_{2}\lambda_{2}(S)}{\lambda_{1}(S)+\lambda_{2}(S)} \\
u_{1} & =-k\lambda_{1}(S)\left( \frac{ \partial p }{ \partial x } +\rho_{1}g\sin\alpha \right) \\
 & =-k\lambda_{1}(S)\left( -g\sin\alpha\frac{\rho_{1}\lambda_{1}(S)+\rho_{2}\lambda_{2}(S)}{\lambda_{1}(S)+\lambda_{2}(S)} +\rho_{1}g\sin\alpha\right) \\
 & =kg\lambda_{1}(S)\sin\alpha\left(  \frac{\rho_{1}\lambda_{1}(S)+\rho_{2}\lambda_{2}(S)}{\lambda_{1}(S)+\lambda_{2}(S)} -\frac{\rho_{1}\lambda_{1}(S)+\rho_{1}\lambda_{2}(S)}{\lambda_{1}(S)+\lambda_{2}(S)}\right) \\
 & =kg\lambda_{1}(s)\sin\alpha \frac{(\rho_{2}-\rho_{1})\lambda_{2}(S)}{\lambda_{1}(S)+\lambda_{2}(S)} \\
 u_{1}& =\Delta\rho kg\sin(\alpha)h(S) 
\end{align}
$$

![[Pasted image 20241208143607.png|800]]
$$
\begin{align}
\phi\frac{ \partial S }{ \partial t } + \frac{ \partial  }{ \partial x } (\Delta\rho kg\sin(\alpha)h(S) ) & =0 \\
\phi \frac{ \partial S }{ \partial t } +\Delta\rho kg\sin(\alpha) \frac{ \partial h(S) }{ \partial x }  & =0 \\
\phi \frac{ \partial S }{ \partial t } +\Delta\rho kg\sin(\alpha) \frac{ \partial h(S) }{ \partial S }\frac{ \partial S }{ \partial x }   & =0 \\
\phi \frac{ \partial S }{ \partial t } +\frac{\Delta\rho kg\sin(\alpha)}{\mu} g'(S)\frac{ \partial S }{ \partial x }   & =0
\end{align}
$$
Set $x\to Lx,t\to Tt$ so
$$
\begin{align}
\frac{\phi}{T}\frac{ \partial S }{ \partial t } +\frac{\Delta\rho kg\sin(\alpha)}{\mu} \frac{g'(S)}{L}\frac{ \partial S }{ \partial x }  & =0 \\
\frac{ \partial S }{ \partial t } +T\frac{\Delta\rho kg\sin(\alpha)}{\mu\phi L}g'(S)\frac{ \partial S }{ \partial x }  & =0
\end{align}
$$
We can choose $T=\frac{\mu_{2}\phi L}{\Delta\rho kg\sin(\alpha)}$ as our time scale to get
$$
\frac{ \partial S }{ \partial t } +g'(S)\frac{ \partial S }{ \partial x } =0
$$
![[Pasted image 20241208150633.png|800]]
$$
S_{0}(x)=\begin{cases}
1 & x<0 \\
0 & x>0
\end{cases}
$$
$$
\begin{align}
\lambda_{i}(S) & = \frac{k_{ri}(S)}{\mu_{i}}\\
g(S) & =\frac{1}{\mu_{2}} \frac{\lambda_{1}(S)\lambda_{2}(S)}{\lambda_{1}(S)+\lambda_{2}(S)} \\
 & =\frac{1}{\mu_{2}} \frac{1}{\mu_{1}\mu_{2}} \frac{S(1-S)}{\frac{S}{\mu_{1}}+\frac{1-S}{\mu_{2}}} \\
 & =\frac{1}{\mu_{2}} \frac{S(1-S)}{\mu_{2}S+\mu_{1}(1-S)} \\
 & =\frac{1}{\mu_{2}} \frac{S-S^2}{\mu_{1}+(\mu_{2}-\mu_{1})S} \\
g'(S) & =\frac{1}{\mu_{2}} \frac{(1-2S)(\mu_{1}+(\mu_{2}-\mu_{1})S)-(S-S^2)(\mu_{2}-\mu_{1})}{(\mu_{1}+(\mu_{2}-\mu_{1})S)^2}
\end{align}
$$
$$
\begin{align}
g'(S) & =\frac{-(1-M)S^2-2MS+M}{((1-M)S+M)^2}
\end{align}
$$
The characteristic for $x_{0}<0$ is then
$$
x(t)=g'(S_{0}(x_{0}))t+x_{0}= \frac{-(1-M)-2M+M}{1}t+x_{0}=-t+x_{0}
$$
for $x_{0}>0$ we have
$$
x(t)=\frac{t}{M}+x_{0}
$$
We get a rarefaction wave between the characteristics
![[Pasted image 20241208153540.png|400]]
As $M<1$, $g'(S)$ is monotonically decreasing between 0 and 1. The solution is therefore continuous as we have a rarefaction wave.

![[Pasted image 20241208154024.png|800]]
![[Pasted image 20241208154049.png|800]]
$f(s)=1-2s$
$$
S_{0}(x)=\begin{cases}
0 & x<0 \\
1 & 0<x<1 \\
0 & 1<x
\end{cases}
$$
The characteristics are for $x<0$ and $x>1$
$$
x(t)=t+x_{0}
$$
and for $0<x<1$
$$
x(t)=-t+x_{0}
$$
have a shock at $x=0$ and $t=0$ and a rarefaction wave.

$F(S)=S-S^2$
The speed of the shock is
$$
\begin{align}
V & =\frac{F(S^-)-F(S^+)}{S^- -S^+} \\
 & = \frac{0-(1-1^2)}{0-1}=0
\end{align}
$$
The rarefaction wave meets the characteristic at $t_{m}=1$
![[Pasted image 20241208154823.png|300]]
![[Pasted image 20241208155006.png|800]]
The speed of the shock now is 
$$
V=\frac{F(S_{R})}{S_{R}}
$$
where $S_{R}$ is the value of the rarefaction wave.
This value can be found as $f^{-1}\left( \frac{x-1}{t} \right)$ 
$$
f(S)=1-2S\implies f^{-1}(S)=\frac{1-S}{2}
$$

and the speed is therefore
$$
\begin{align}
V & =\frac{F\left( f^{-1}\left( \frac{x-1}{t} \right) \right)}{f^{-1}\left( \frac{x-1}{t} \right)} \\
 & = \frac{F\left( \frac{1}{2}-\frac{x-1}{2t}\right)}{\frac{1}{2}-\frac{x-1}{2t}} \\
 & = \frac{\left( \frac{1}{2}-\frac{x-1}{2t} \right)\left( 1-\frac{1}{2}+\frac{x-1}{2t} \right)}{\frac{1}{2}-\frac{x-1}{2t}} \\
 & =\frac{1}{2}+\frac{x-1}{2t} \\
a' & =\frac{1}{2}+ \frac{a-1}{2t}
\end{align}
$$
and the initial $a(1)=0$ since it starts at $x=0$ at $t=1$ 

![[Pasted image 20241208161011.png|800]]
$$
S_{R}=f^{-1}\left( \frac{a(t)-1}{t} \right)= \frac{1-\frac{a(t)-1}{t}}{2}=\frac{1}{2}-\frac{a(t)-1}{2t}
$$

$$
S_{R}=\frac{1}{2}-\frac{t-2\sqrt{ t }}{2t}=\frac{1}{2}-\frac{1}{2}+ \frac{1}{\sqrt{ t }}=\frac{1}{\sqrt{ t }}
$$
![[Pasted image 20241208161731.png|800]]
$$
\begin{align}
f(u,\mu) & =(u-\mu)(u^2-\mu) \\
\frac{ \partial f }{ \partial u }  & =u^2-\mu+2u(u-\mu)=3u^2-2u\mu-\mu=u(3u-2\mu)-\mu
\end{align}
$$

It is clear that one equilibrium points are when $u= \mu$. Inserting $u=\mu$ into $\frac{ \partial f }{ \partial u }$:
$$
3u^2-2u^2-u=u^2-u=u(u-1)
$$
here, $\frac{ \partial f }{ \partial u }<0$ when $0<u<1$. 

The other equilibrium points are when $u=\pm \sqrt{ \mu }$ inserting
$$
3\mu \mp2\mu^{3/2}-\mu=2\mu(1\mp \sqrt{ \mu }),
$$
so this is only stable when $u=+\sqrt{ \mu }$ and $1<u$.

![[Pasted image 20241208163547.png|800]]
![[Pasted image 20241208163600.png|800]]
$\kappa$ is death rate, $\beta$ is birth rate when there is no inhibitor, $\gamma$ is the resistivity against the inhibitor, $\eta$ is the production of the inhibitor while $\lambda$ is the death rate of the inhibitor.

Let $t\to \frac{1}{\kappa}t$, $u\to Uu,v\to Vv$ so
$$
\begin{align}
\kappa U\frac{ \partial u }{ \partial t }  & = \frac{\beta}{1+\frac{Vv}{\gamma}}Uu-\kappa Uu \\
\frac{ \partial u }{ \partial t }  & =\frac{\frac{\beta}{\kappa}}{1+\frac{ V}{\gamma}v}u-u \\
\kappa V\frac{ \partial v }{ \partial t }  & =\eta Uu-\lambda Vv \\
\frac{\kappa}{\lambda} \frac{ \partial v }{ \partial t }  & =\frac{\eta U}{\lambda V}u-v
\end{align}
$$
We set $V=\gamma$ and $U=\frac{\gamma\lambda}{\eta}$ such that
$$
\begin{align}
\frac{ \partial u }{ \partial t }  & =\frac{\alpha}{1+v}u-u \\
\epsilon\frac{ \partial v }{ \partial t }  & =u-v
\end{align}
$$
where $\alpha=\frac{\beta}{\kappa}$ is the cells birth rate divided by the cells death rate, and $\epsilon=\frac{\kappa}{\lambda}$ is the death rate of cells divided by the death rate of the inhibitor.

$\alpha>1$ makes sense as the birth rate would be larger than the death rate. Since $k\ll \lambda$ then $\epsilon\ll1$.

Setting $\frac{ \partial u }{ \partial t }=\frac{ \partial v }{ \partial t }=0$ gives $u=v$ and
$$
\begin{align}
0 & =\frac{\alpha}{1+u}u-u
\end{align}
$$
which has the solution $(u,v)=(0,0)$ and
$$
\begin{align}
0 & =\frac{\alpha}{1+u}-1 \\
1+u & =\alpha \\
v=u & =\alpha-1
\end{align}
$$
The jacobian is
$$
J=\begin{bmatrix}
\frac{\alpha}{1+v}-1 & -\frac{\alpha}{(1+v)^2}u \\
\frac{1}{\epsilon} & -\frac{1}{\epsilon}
\end{bmatrix}
$$
For $u=v=0$, the jacobian is
$$
\begin{align}
J(0,0) & =\begin{bmatrix}
\alpha-1 & 0 \\
\frac{1}{\epsilon} & -\frac{1}{\epsilon}
\end{bmatrix} \\
J(\alpha-1,\alpha-1) & =\begin{bmatrix}
0 & -\frac{\alpha-1}{\alpha} \\
\frac{1}{\epsilon} & -\frac{1}{\epsilon}
\end{bmatrix}
\end{align}
$$
$\det(0,0)=\frac{1-\alpha}{\epsilon}<0$ since $\alpha>1$ so this equilibrium point is unstable.
$\det J(\alpha-1,\alpha-1)=\frac{\alpha-1}{\alpha\epsilon}>0$ and $\mathrm{Tr}J=-\frac{1}{\epsilon}$ so this equilibrium point is asymptomatically stable.

![[Pasted image 20241208175737.png|800]]
$$
\begin{align}
\frac{ \partial u }{ \partial t }  & =\frac{\alpha}{1+v}u-u \\
\epsilon\frac{ \partial v }{ \partial t }  & =u-v
\end{align}
$$
Let $\epsilon\to0$ 
$$
\begin{align}
\frac{ \partial u }{ \partial t }  & =\frac{\alpha}{1+v}u-u \\
u & =v \\
\frac{ \partial u }{ \partial t }  & =\frac{\alpha}{1+u}u-u \\
\frac{\text{d}u}{\text{d}t}  & =\left( \frac{\alpha-1-u}{1+u} \right)u \\
\int\frac{1+u}{(\alpha-1-u)u}\text{ d} u & =\int\text{ d} t
\end{align}
$$
delbrøksoppspalting<3
$$
\begin{align}
\frac{1+u}{(\alpha-1-u)u} & =\frac{A}{\alpha-1-u}+\frac{B}{u} \\
1+u & =Au+B\alpha-B-Bu \\
1+u & =B\alpha-B+(A-B)u \\
\begin{cases}
B\alpha-B=1 \\
A-B =1
\end{cases}
\end{align}
$$
$B(\alpha-1)=1\implies B=\frac{1}{\alpha-1}$ and $A=1+B=\frac{\alpha}{\alpha-1}$. So
$$
\frac{1+u}{(\alpha-1-u)u}=\frac{1}{\alpha-1}\left( \frac{\alpha}{\alpha-1-u}+\frac{1}{u} \right)
$$

$$
\begin{align}
\frac{1}{\alpha-1}\int\left( \frac{\alpha}{\alpha-1-u}+\frac{1}{u} \right)\text{ d} u & =\int \text{ d} t \\
\frac{1}{\alpha-1}(-\alpha \ln|\alpha-1-u|+\ln u ) & =t+C \\
\ln\left( \frac{u}{|\alpha-1-u|^\alpha} \right) & =(\alpha-1)t+C \\
\frac{u}{|\alpha-1-u|^\alpha} & =Ce^{ (\alpha-1)t }
\end{align}
$$
Since $\alpha>1$, there is a positive exponent on the right hand side. So when $t\to \infty$, the RHS$\to \infty$ if $C\neq0$. Then the LHS also has to go to infinity, which happens when 
$$u\to\alpha-1
$$
![[Pasted image 20241208182217.png|800]]
![[Pasted image 20241208182230.png|800]]

$$
\begin{align}
\frac{1}{\delta(\epsilon)}\frac{ \partial u }{ \partial t }  & =\frac{\alpha}{1+v}u-u \\
\frac{\epsilon}{\delta(\epsilon)}\frac{ \partial v }{ \partial t }  & =u-v
\end{align}
$$
let $\delta(\epsilon)=\epsilon$ and 
$$
\begin{align}
\frac{1}{\epsilon}\frac{ \partial u }{ \partial t }  & =\frac{\alpha}{1+v}u-u \\
\frac{ \partial v }{ \partial t }  & =u-v
\end{align}
$$
let $\epsilon\to0$ and
$$
\begin{align}
\frac{ \partial u }{ \partial t }  & =0 \\
\frac{ \partial v }{ \partial t }  & =u-v
\end{align}
$$
Then $u=C_{1}$ is constant and
$$
\begin{align}
\frac{ \partial v }{ \partial \tau }  & =u_{0}-v \\
v'+v & =C_{1} \\
v'e^{ t }+v e^{ \tau } & =u_{0}e^{ \tau } \\
\int(v e^{ t })'\text{ d} \tau & =\int u_{0}e^{ \tau } \text{ d} \tau \\
v e^{ t } & =u_{0}e^{ \tau }+C_{2} \\
v(\tau) & =u_{0}+C_{2}e^{ -\tau } \\
v(0) & =u_{0}+C_{2}=v_{0} \\
v(\tau) & =u_{0}+(v_{0}-u_{0})e^{ -\tau }
\end{align}
$$
We also have that $u(\tau)=u_{0}$. The uniform solutions are
$$
\begin{align}
u(t) & =u_{O}(t)+u_{I}\left( \frac{t}{\epsilon} \right)-\lim_{ t \to \infty } u_{I}(t) \\
u(t) & =u_{O}(t)+u_{0}-u_{0}=u_{O}(t) \\
v(t) & =u_{O}(t)+v_{I}\left( \frac{t}{\epsilon} \right)-\lim_{ \tau \to \infty } v_{I}(\tau)  \\
 & =u_{O}(t)+u_{0}+\left(v_{0}-u_{0}\right)e^{ -t/\epsilon }-u_{0} \\
 & =u_{O}(t)+\left(v_{0}-u_{0}\right)e^{ -t/\epsilon }
\end{align}
$$


