![[Pasted image 20241129134941.png|800]]
$[A]=m^2$, $[\mu ]=kgs^{-1}m^{-1}$, $[\rho ]=kg m^{-3}$, $[v]=ms^{-1}$, $[F]=kg ms^{-2}$.
We have three units and five variables, and 
$$\begin{bmatrix} & A & \mu  & \rho  & v & F \\ m & 2 & -1 & -3 & 1 & 1 \\ s & 0 & -1 & 0 & -1 & -2 \\ kg & 0 & 1 & 1 & 0 & 1\end{bmatrix}$$
Any variables except for $F$ can be chosen to be the three core variables. Let's choose $A,\mu ,v$.
We need to find two dimensionless variables, one containing $F$ and one not containing $F$. Let's first find the one containing $F$:
$$\begin{aligned}
F&= \mathrm{kgms^{-2}}\\
\frac{F}{\mu }&= \mathrm{\frac{kgms^{-2}}{kgs^{-1}m^{-1}}}=\mathrm{m^{2}s^{-1}}\\
\frac{F}{\mu v}&= \mathrm{\frac{m^{2}s^{-1}}{ms^{-1}}=m}\\
\frac{F}{\mu v \sqrt{A}}&= 1.
\end{aligned}$$
So we set $\pi _1=\frac{F}{\mu v \sqrt{A}}$.
Start by eliminating kg
$$\begin{aligned}
\left[\frac{\rho }{\mu  }\right]&= \mathrm{\frac{kgm^{-3}}{kgs^{-1}m^{-1}}}=\mathrm{m^{-2}s}\\
\left[\frac{\rho v}{\mu  }\right]&= \mathrm{m^{-2}s \cdot ms^{-1}}=m^{-1}\\
\left[\frac{\rho v \sqrt{A}}{\mu  }\right]&= \mathrm{m^{-1}\cdot m}=1
\end{aligned}$$
So we set
$$\pi_{2} = \frac{\rho v \sqrt{A}}{\mu }$$

Now we can set the expression
$$\begin{aligned}
f(\pi _{1},\pi _{2}, A,v,\mu )&=  0,\\
f(\pi _{1},\pi _{2})&= 0
\end{aligned}$$
and since $\pi _{1}= h(\pi _{2})$,
$$\begin{aligned}
\frac{F}{\mu v \sqrt{A}}&= h \left(\frac{\rho v \sqrt{A}}{\mu } \right)\\
F&= \mu v \sqrt{A}\cdot h \left(\frac{\rho v \sqrt{A}}{\mu } \right)
\end{aligned}$$
```ad-question
Suppose you had a (high) tank of water and a number of spheres of different masses m1, m2, . . . , mN with corresponding cross-sectional areas A1, A2, . . . , AN . All spheres have higher mass density than the fluid. Describe how you would estimate (knowing the mass density and viscosity of water) N function values of h through actual measurements.

```

$$\frac{F}{\mu v \sqrt{A}}= h \left(\frac{\rho v \sqrt{A}}{\mu } \right)$$
We know $\mu ,\rho$ and have $A_{1}\dots ,A_{N}$ and $m_{1},\dots m_{N}$. We can measure the velocity for the different spheres and get $v_{1},\dots v_{N}$.


![[Pasted image 20241129135010.png|800]]
Setting the derivatives to zero:
$$\begin{aligned}
0&= u^{2}-v^{2}+3\\
0&= -u^{2}+v+3\\
\text{adding}\\
0&= v^{2}-v-6\\
0&= (v-3)(v+2)
\end{aligned}$$
For $u$:
$$\begin{aligned}
u&= \sqrt{v+3}\\
u_{1}&= \pm \sqrt{6}\\
u_{2}&= \pm 1
\end{aligned}$$
The two equilibrium points are $(u,v)=(\sqrt{6},3)$, $(-\sqrt{6},3)$, $(1,-2)$ and $(-1,-2)$.
Let $\mathbf x=\begin{bmatrix}u \\ v\end{bmatrix}$ such that
$$\frac{\text{d}\mathbf x}{\text{d}t}=\mathbf f(\mathbf x),\qquad \mathbf f(\mathbf x)=\begin{bmatrix}u^{2}-v^{2}+3 \\ -u^{2}+v+3\end{bmatrix}$$
Jacobi:
$$J(u,v)=\begin{bmatrix}2u & -2v \\ -2u & 1\end{bmatrix}$$
Stability of equilibrium points:
1. If $\det J(\mathbf x_{e})<0\quad\implies\quad$ unstable
2. If $\det J(\mathbf x_{e})>0$
	1. $\text{trace} J(\mathbf x_{e})>0\quad\implies\quad$ unstable
	2. $\text{trace} J(\mathbf x_{e})<0\quad\implies\quad$ asymptomatically stable
	3. $\text{trace} J(\mathbf x_{e})=0\quad\implies\quad$ stable

$$J(\pm\sqrt{6},3)=\begin{bmatrix}\pm2\sqrt{6}  & -6 \\ \mp2\sqrt{6} & 1\end{bmatrix}$$
$\det J=\pm 2\sqrt{6} \pm12 \sqrt{6}$ unstable for $(\sqrt{6},3)$. 
And $\text{trace} J(-\sqrt{6},3)=-2\sqrt{ 6 }\cdot 1<0\implies$ stable.
$$
J(\pm1,-2)=\begin{bmatrix}
\pm1 & 2 \\
\mp1 & 1
\end{bmatrix}
$$
$\det J(\pm1,-2)=\pm1\pm2$ 
so $J(-1,-2)$ is unstable
$\mathrm{Tr}J(1,-2)=2$ so unstable.
Only stable eq point is $(-\sqrt{ 6 },3)$.



![[Pasted image 20241129135023.png|800]]
### Outer solution
Since we are at the outer solution, we use the BC $y(1)=\frac{1}{2}$. Setting $y=y_{0}+\epsilon y_{1}$:
$$
\begin{align}
\epsilon(y''_{0}+\epsilon y_{1}'')+y_{0}'+\epsilon y_{0}'+2x(y_{0}+\epsilon y_{1})^3 & = 0\\
\epsilon y_{0}''+y_{0}'+\epsilon y_{0}'+2x(y_{0}^3+2\epsilon y_{0}^2y_{1}) & =0 \\
(y_{0}'+2xy_{0}^3) & =0 \\
\frac{y_{0}'}{y_{0}^3} & =-2x \\
\int \frac{1}{y_{0}^3}\text{ d} y_{0} & =\int-2x\text{ d} x \\
-\frac{1}{2y_{0}^2} & =-x^2+C \\
\text{setting }y(1)=\frac{1}{2}\qquad -\frac{1}{2\left( \frac{1}{2} \right)^2} & =-1+C \\
C & =1-2=-1 \\
-\frac{1}{2y^2_{0}} & =-x^2-1 \\
y_{0}^2 & =\frac{1}{2(x^2+1)} \\
y_{0} & =\frac{1}{\sqrt{ 2(x^2+1) }}
\end{align}
$$
### Inner solution
Since the boundary layer is at $x=0$, we can set $\eta=\frac{x}{\delta(\epsilon)}$. Postulate
$$
y(x)=Y\left( \frac{x}{\delta(\epsilon)} \right)
$$
Then
$$
\begin{align}
\epsilon \frac{ \partial ^2Y }{ \partial x^2 } +\frac{ \partial Y }{ \partial x } +2xY^3 & =0 \\
\frac{\epsilon}{\delta(\epsilon)^2}Y''+\frac{1}{\delta(\epsilon)}Y'+2xY^3 & =0
\end{align}
$$
let $\delta(\epsilon)=\epsilon$:
$$
\begin{align}
\frac{1}{\epsilon}Y''+\frac{1}{\epsilon}Y'+2\epsilon\eta Y^3 & =0 \\
Y''+Y'+2\epsilon^2\eta Y^3 & =0
\end{align}
$$
For 0th order,
$$
\begin{align}
Y''+Y' & =0 \\
\lambda^2+\lambda & =0 \\
\lambda=-1 \vee\lambda & =0 
\end{align}
$$
so solution is
$$
\begin{align}
Y(\eta) & =C_{1}e^{ \lambda_{1} \eta }+C_{2}e^{ \lambda_{2}\eta } \\
 & =C_{1}+C_{2}e^{ -\eta } \\
Y(0) & =0 \\
C_{1}+C_{2} & =0 \\
Y(\eta) & =C_{1}(1-e^{ -\eta })
\end{align}
$$
Matching condition:
$$\lim_{\eta  \to \infty}Y(\eta )= \lim_{x \to 0}y(x)$$
$$
\begin{align} 
\lim_{ \eta \to \infty } C_{1}(1-e^{ -\eta }) & =\lim_{ x \to 0 } \frac{1}{\sqrt{ 2(x^2+1) }} \\
C_{1} & =\frac{1}{\sqrt{ 2 }}
\end{align}
$$
So 
$$
Y(\eta)= \frac{1-e^{ -\eta }}{\sqrt{ 2 }}
$$

Uniform solution:
$$
\begin{align}
y^u & = y(x)+Y\left(\frac{x}{\varepsilon }\right)-\lim_{x \to 0}y(x) \\
 & =\frac{1}{\sqrt{ 2(x^2+1) }}+\frac{1-e^{ -\eta }}{\sqrt{ 2 }}-\frac{1}{\sqrt{ 2 }} \\
 & =\frac{1}{\sqrt{ 2 }}\left( \frac{1}{\sqrt{ x^2+1 }}-e^{ -x/\epsilon } \right)
\end{align}
$$


![[Pasted image 20241129135605.png|800]]
![[Pasted image 20241129135617.png|800]]
The reproduction rate of the rabbits $\alpha x$, is proportional to the population of rabbits with proportionality constant $\alpha$, which can be interpreted as the natural growth coefficient. 
$\beta$ is the hunting rate of the foxes.
$\delta$  is the reproduction rate of foxes.
$\gamma$ is natural death rate of foxes.

Let $x \to Xx$ and $y\to Yy$ and $t\to Tt$. Then,
$$
\begin{align}
\frac{X}{T}\frac{\text{d}x}{\text{d}t}  & =\alpha Xx-\beta XYxy \\
\frac{Y}{T}\frac{\text{d}y}{\text{d}t}  & =\delta XYxy-\gamma Yy \\
\frac{\text{d}x}{\text{d}t}  & =\alpha Tx-\beta YTxy \\
\frac{\text{d}y}{\text{d}t}  & =\delta XTxy-\gamma Ty
\end{align}
$$
So set $T=\frac{1}{\alpha}$ and $Y=\frac{\alpha}{\beta}$ such that
$$
\begin{align}
\frac{\text{d}x}{\text{d}t}  & =x-xy \\
\frac{\text{d}y}{\text{d}t}  & =\frac{\delta X}{\alpha}xy-\frac{\gamma}{\alpha}y
\end{align}
$$
finally we choose $X=\frac{\alpha}{\delta}$ such that
$$
\begin{align}
\frac{\text{d}x}{\text{d}t}  & =x-xy \\
\frac{\text{d}y}{\text{d}t}  & =xy-\eta y
\end{align}
$$
here $\eta=\frac{\gamma}{\alpha}$. 


![[Pasted image 20241129135635.png|800]]

$$
\begin{align}
\frac{\text{d}(\eta+\epsilon \tilde{x}(t))}{\text{d}t}  & = \eta+\epsilon \tilde{x}(t)-(\eta+\epsilon \tilde{x}(t))(1+\epsilon \tilde{y}(t)) \\
\frac{\text{d}(1+\epsilon \tilde{y}(t))}{\text{d}t}  & =(\eta+\epsilon \tilde{x}(t))(1+\epsilon \tilde{y}(t))-\eta (1+\epsilon \tilde{y}(t)) \\
\epsilon\frac{\text{d}x}{\text{d}t}  & = \eta+\epsilon x(t)-\eta-\eta\epsilon y(t)-\epsilon x(t)-\epsilon^2x(t)y(t) \\
\epsilon \frac{\text{d}y}{\text{d}t}  & = \eta+\eta\epsilon y(t)+\epsilon x(t)+\epsilon^2x(t)y(t)-\eta-\eta\epsilon y(t) \\
\frac{\text{d}x}{\text{d}t}  & =-\eta y-\epsilon xy \\
\frac{\text{d}y}{\text{d}t}  & =x+\epsilon xy
\end{align}
$$

we ignore $\epsilon$ and get the linear system

$$
\frac{\text{d}}{\text{d}t} \begin{bmatrix}
x \\
y
\end{bmatrix}=\begin{bmatrix}
0 & -\eta \\
1 & 0
\end{bmatrix}\begin{bmatrix}
x \\
y
\end{bmatrix}
$$
For a linear system of the form
$$
\frac{\text{d}}{\text{d}t} \vec{x}=\mathbf{A}\vec{x},
$$
the solutions are of the form
$$
\vec{x}=C_{1}\vec{x}_{1}e^{ \lambda_{1} t }+C_{2}\vec{x}_{2}e^{ \lambda_{2}t }
$$
where $\vec{x}_{1},\vec{x}_{2}$ are the eigenvectors and $\lambda_{1},\lambda_{2}$ are the eigenvalues.

The eigenvalues can be found as
$$
\begin{align*}
\det\begin{bmatrix}
\lambda & \eta \\
-1 & \lambda 
\end{bmatrix} & =0 \\
\lambda^{2}+\eta & =0 \\
\lambda & =\pm i\sqrt{ \eta }
\end{align*}
$$
so the solution is of the form
$$
\vec{x}=C_{1}\vec{x}_{1}e^{ i\sqrt{ \eta }t }+C_{2}\vec{x}_{2}e^{ -i\sqrt{ \eta }t }
$$
$f(u)=e^{ \pm iu }$ has minimal period $2\pi$ so we have
$$
\begin{align}
\sqrt{ \eta }\tau & =2\pi \\
\tau & =\frac{2\pi}{\sqrt{ \eta }}
\end{align}
$$
the physical period is then
$$
T\tau=T2\pi \sqrt{ \frac{\alpha}{\gamma} }=\frac{2\pi}{\sqrt{ \alpha\gamma }}
$$
![[Pasted image 20241206142842.png|800]]
![[Pasted image 20241206144458.png|800]]
The flux of cars is the velocity times the amount of cars:
$$
J(u) =uv(u)=uv_{m}\left( 1-\frac{u}{u_{m}} \right)
$$
The 
$$
\begin{align}
\frac{\text{d}}{\text{d}t} \int_{V}u\text{ d} V  +\int_{A}J(u)\cdot \mathbf{n}\text{ d} A & = 0\\
\int_{V}\frac{\text{d}u}{\text{d}t} \text{ d} V +\int_{V}\nabla \cdot J\text{ d} V& = 0\\
\frac{\text{d}u(x,t)}{\text{d}t} +\frac{ \partial J(u(x,t)) }{ \partial x }  & =0 \\
\frac{\text{d}u}{\text{d}t} +\frac{ \partial  }{ \partial x } \left( v_{m}\left( u-\frac{u^2}{u_{m}} \right) \right) & =0 \\
\frac{ \partial u }{ \partial t } +v_{m}\frac{ \partial  }{ \partial x } \left( u-\frac{u^2}{u_{m}} \right) & =0
\end{align}
$$
Let $x\to Lx$, $t\to \frac{L}{v_{m}}t$ and $u\to u_{m}u$ such that
$$
\begin{align}
\frac{u_{m}v_{m}}{L}\frac{ \partial u }{ \partial t } +\frac{v_{m}}{L}\frac{ \partial  }{ \partial x } (u_{m}u-u_{m}u^2) & =0 \\
\frac{ \partial u }{ \partial t } +\frac{ \partial  }{ \partial x } (u-u^2) & =0 \\
\frac{ \partial u }{ \partial t } +\frac{ \partial u }{ \partial x } -2u \frac{ \partial u }{ \partial x }  & =0 \\
\frac{ \partial u }{ \partial t } +(1-2u)\frac{ \partial u }{ \partial x }  & =0
\end{align}
$$
The initial values becomes
$$
\begin{align}
u(x,0)=\begin{cases}
1 & x<0 \\
1-x & 0<x<1 \\
0 & x>1
\end{cases}
\end{align}
$$
![[Pasted image 20241206145352.png|800]]
$$
f(u)=1-2u
$$
For $x_{0}<0$, 
$$
\begin{align}
x(t) & =f(u(x_{0},t_{0}))t+x_{0} \\
x(t) & =(1-2)t+x_{0} \\
 & =x_{0}-t
\end{align}
$$
For $0<x_{0}<1$,
$$
\begin{align}
x(t) & =f(u(x_{0},t_{0}))t+x_{0}  \\
x(t) & =(1-2(1-x_{0}))t+x_{0} \\
 & =(2x_{0}-1)t+x_{0}
\end{align}
$$
For $x_{0}>1$,
$$
\begin{align}
x(t) & =(1-2\cdot0)t+x_{0} \\
 & =t+x_{0}
\end{align}
$$

![[Pasted image 20241206160059.png|500]]
There are no shocks or rarefaction waves.
For $x<-t$, we see that $u(x,t)=1$. 
For $x>1+t$, we see that $u(x,t)=0$.
For $-t<x<1+t$, we solve for for $x_{0}$ in
$$
\begin{align}
x & =(2x_{0}-1)t+x_{0} \\
x & =(2t+1)x_{0}-t \\
x_{0} & =\frac{x+t}{2t+1}
\end{align}
$$
So 
$$
\begin{align}
u(x,t) & =u_{0}(x_{0}(x,t)) \\
 & =1-\frac{x+t}{2t+1} \\
 & =\frac{t+1-x}{2t+1}
\end{align}
$$
in summary
$$
u(x,t)=\begin{cases}
1 & x<-t \\
\frac{t+1-x}{2t+1} & -t<x<1+t \\
0 & 1+t<x
\end{cases}
$$
![[Pasted image 20241206161109.png|800]]
The car will stay at $x=-1$ until it meets the characteristic $x=-t$ when $t=1$.
So
$$
y(t)=\begin{cases}
-1 & t<1 \\
\vdots
\end{cases}
$$


$$
\begin{align}
\frac{\text{d}y}{\text{d}t}  & =v(u(y(t),t)) \\
\frac{\text{d}y}{\text{d}t}  & =1-u(y(t),t) \\
\frac{\text{d}y}{\text{d}t}  & =1-\frac{t+1-y(t)}{2t+1} \\
y' & = \frac{t+y}{2t+1} \\
y'-\frac{y}{2t+1} & =\frac{t}{2t+1}
\end{align}
$$

$$
\begin{align}
p(t) & =\int- \frac{1}{2t+1}\text{ d} t=-\frac{1}{2}\ln(2t+1) \\
 e^{ p(t) } & =e^{ -1/2\ln(2t+1) }=e^{ \ln(2t+1)^{-1/2} }=(2t+1)^{-1/2}
\end{align}
$$
multiply by this guy
$$
\begin{align}
y'(2t+1)^{-1/2}-y(2t+1)^{-3/2} & =t(2t+1)^{-3/2} \\
y(2t+1)^{-1/2} & =\int t(2t+1)^{-3/2}\text{ d} t \\
y(2t+1)^{-1/2} & =\frac{1}{2} ((2t+1)^{1/2}+(2t+1)^{-1/2})+C \\
y(t) & =\frac{1}{2}(2t+1+1)+C(2t+1)^{1/2} \\
y(t) & =t+1+C(2t+1)^{1/2} \\
y(1) & =2+C\sqrt{ 3 }=-1 \\
C & =-\frac{3}{\sqrt{ 3 }}=-\sqrt{ 3 } \\
y(t) & =t+1-(6t+3)^{1/2}
\end{align}
$$
since $y<t+1$, we never reach the other domain.

![[Pasted image 20241206170316.png|800]]
$$
\begin{align}
\frac{\text{d}}{\text{d}t} \int_{V}\rho(p)\phi(p) \text{ d} V+\int_{A}\rho(p)\vec{q}\cdot \vec{n}\text{ d} A & =0 \\
\int_{V}\phi \frac{\text{d}\rho}{\text{d}t} +\rho \frac{\text{d}\phi}{\text{d}t} \text{ d} V+\int_{V}\nabla \cdot(\rho \vec{q})\text{ d} V & =0 \\
\phi \frac{\text{d}\rho}{\text{d}t} +\rho \frac{\text{d}\phi}{\text{d}t} -\frac{k}{\mu}\nabla \cdot(\rho \nabla p) & =0 \\
\phi \frac{\text{d}\rho}{\text{d}t} +\rho \frac{\text{d}\phi}{\text{d}t} -\frac{k}{\mu}\left( \frac{ \text{d} \rho }{ \text{d} p } \nabla p\cdot \nabla p+\rho \nabla^2p   \right) & =0
\end{align}
$$
Each term:
$$
\begin{align}
\frac{ \text{d} \rho }{ \text{d} t }  & =\rho_{0}c_{f}\frac{ \partial p }{ \partial t }e^{ c_{f}(p-p^{(0)}) }  \\
\frac{ \text{d} \phi }{ \text{d} t }  & =\phi_{0}c_{r}\frac{ \partial p }{ \partial t }e^{ c_{r}(p-p^{(0)}) }  \\
\frac{ \text{d} \rho }{ \text{d} p  }  & =\rho_{0}c_{f}e^{ c_{f}(p-p^{(0)}) }
\end{align}
$$
$$
\begin{align}
\phi \frac{\text{d}\rho}{\text{d}t} +\rho \frac{\text{d}\phi}{\text{d}t}  & =\phi_{0}e^{ c_{r}(p-p^{(0)}) }\rho_{0}c_{f}\frac{ \partial p }{ \partial t } e^{ c_{f}(p-p^{(0)}) }+\rho_{0}e^{ c_{f}(p-p^{(0)}) }\phi_{0}c_{r}\frac{ \partial p }{ \partial t } e^{ c_{r}(p-p^{(0)}) } \\
 & =\frac{ \partial p }{ \partial t } e^{ c_{r}(p-p^{(0)}) }e^{ c_{f}(p-p^{(0)}) }\rho_{0}\phi_{0}(c_{r}+c_{f}) \\
& =\frac{ \partial p }{ \partial t } e^{ c_{r}(p-p^{(0)}) }e^{ c_{f}(p-p^{(0)}) }\rho_{0}\phi_{0}c_T
\end{align}
$$
$$
\begin{align*}
\phi \frac{\text{d}\rho}{\text{d}t} +\rho \frac{\text{d}\phi}{\text{d}t}  & =\frac{k}{\mu}\left( \frac{ \text{d} \rho }{ \text{d} p } \nabla p\cdot \nabla p+\rho \nabla^2p   \right) \\
\frac{ \partial p }{ \partial t } e^{ c_{r}(p-p^{(0)}) }e^{ c_{f}(p-p^{(0)}) }\rho_{0}\phi_{0}c_T & =\frac{k}{\mu}\left(\rho_{0}c_{f}e^{ c_{f}(p-p^{(0)}) } \nabla p\cdot \nabla p+\rho_{0}e^{ c_{f}(p-p^{(0)}) } \nabla^2p   \right)  \\
\frac{ \partial p }{ \partial t }e^{ c_{r}(p-p^{(0)}) }e^{ c_{f}(p-p^{(0)}) }  & =\frac{k}{\mu \phi_{0}c_{T}}e^{ c_{f}(p-p^{(0)}) }(c_{f}\nabla p\cdot \nabla p+\nabla^2p) \\
\frac{ \partial p }{ \partial t }  & =\frac{k}{\mu \phi_{0}c_{T}}e^{ -c_{r}(p-p^{(0)}) }(c_{f}\nabla p\cdot \nabla p+\nabla^2p)
\end{align*}
$$
![[Pasted image 20241207103950.png|800]]
$$
\frac{ \partial p }{ \partial t }   =\frac{k}{\mu \phi_{0}c_{T}}e^{ -c_{r}(p-p^{(0)}) }(c_{f}\nabla p\cdot \nabla p+\nabla^2p)
$$
Let $p\to p^{(0)}+p\Delta p$, and $x\to Lx$ and $t\to Tt$. Then the equation becomes
$$
\begin{align}
\frac{\Delta p}{T}\frac{ \partial p }{ \partial t }    & =\frac{k}{\mu \phi_{0}c_{T}}e^{ -c_{r}p\Delta p }\left( c_{f} \frac{\Delta p}{L}\frac{ \partial p }{ \partial x } \cdot \frac{\Delta p}{L}\frac{ \partial p }{ \partial x } +\frac{\Delta p}{L^2}\frac{ \partial ^2p }{ \partial x^2 }  \right) \\
\frac{ \partial p }{ \partial t }  & =\frac{kT}{\mu\phi_{0}c_{T}L^2}e^{ -(c_{r}\Delta p)p }\left( c_{f}\Delta p\left( \frac{ \partial p }{ \partial x }  \right)^2+\frac{ \partial ^2p }{ \partial x^2 }  \right)
\end{align}
$$
Let $T=\frac{L^2\mu\phi_{0}c_{T}}{k}$, and denote $\epsilon=c_{r}\Delta p$ and $a=\frac{c_{f}}{c_{r}}$ such that
$$
\frac{ \partial p }{ \partial t } =e^{ -\epsilon p }\left( a\epsilon\left( \frac{ \partial p }{ \partial x }  \right)^2+\frac{ \partial ^2p }{ \partial x^2 }  \right)
$$
Use Taylor series for $e^{ u }$:
$$
\frac{ \partial p }{ \partial t } =\left( 1-\epsilon p+\frac{\epsilon^2p^2}{2}+\dots \right)\left( a\epsilon\left( \frac{ \partial p }{ \partial x }  \right)^2+\frac{ \partial ^2p }{ \partial x^2 }  \right)
$$

Let $p(x,t)=p_{0}(x,t)+\epsilon p_{1}(x,t)$ such that
$$
\begin{align}
\frac{ \partial p_{0} }{ \partial t }+\epsilon \frac{ \partial p_{1} }{ \partial t }   & =(1-\epsilon p_{0})\left( a\epsilon\left(  \frac{ \partial p_{0} }{ \partial x }  \right)^2+\frac{ \partial ^2p_{0} }{ \partial x^2 }+\epsilon \frac{ \partial ^2p_{1} }{ \partial x^2 }   \right)+\mathcal{O}(\epsilon^2) \\
\frac{ \partial p_{0} }{ \partial t }+\epsilon \frac{ \partial p_{1} }{ \partial t }   & = a\epsilon\left(  \frac{ \partial p_{0} }{ \partial x }  \right)^2+\frac{ \partial ^2p_{0} }{ \partial x^2 }+\epsilon \frac{ \partial ^2p_{1} }{ \partial x^2 }-\epsilon p_{0}\frac{ \partial ^2p_{0} }{ \partial x^2 } +\mathcal{O}(\epsilon^2)
\end{align}
$$
zeroth order is
$$
\frac{ \partial p_{0} }{ \partial t }=\frac{ \partial ^2p_{0} }{ \partial x^2 }  
$$
First order is
$$
\frac{ \partial p_{1} }{ \partial t } =a\left( \frac{ \partial p_{0} }{ \partial x }  \right)^2+\frac{ \partial^2 p_{1} }{ \partial x^2 } -p_{0}\frac{ \partial^2 p_{0} }{ \partial x^2 } 
$$
The unscaled boundary conditions were
$$
p(0,t)=p^{(1)},\qquad p(L,t)=p^{(0)}
$$
the scaled becomes
$$
\begin{align}
p(0,t) & =1\implies \quad p_{0}(0,t)=1,\qquad p_{1}(0,t)=0 \\
p(1,t) & =0 \implies \quad p_{0}(1,t)=0,\qquad p_{1}(1,t)=0
\end{align}
$$
and the scaled initial values are
$$
p(x,0)=0\implies \quad p_{0}(x,0)=0 \qquad p_{1}(x,0)=0
$$


![[Pasted image 20241207103958.png|500]]
