The recurrence relation given is $a_n = 4 - a_{n-1} + a_{n-1} \cdot a_{n-2}$ for $n > 2$. Simplifying this, we can rewrite it as $a_n = 4 - a_{n-1}(1 - a_{n-2})$. Using the initial values $a_1 = 1$ and $a_2 = 1$, we calculate $a_3$ as follows: $a_3 = 4 - a_2(1 - a_1) = 4 - 1(1 - 1) = 4$.

Next, we find $a_4$: $a_4 = 4 - a_3(1 - a_2) = 4 - 4(1 - 1) = 4$. Observing that $a_3$ and $a_4$ are both 4, we proceed to calculate $a_5$: $a_5 = 4 - a_4(1 - a_3) = 4 - 4(1 - 4) = 4 - 4(-3) = 16$.

Continuing, we calculate $a_6$: $a_6 = 4 - a_5(1 - a_4) = 4 - 16(1 - 4) = 4 - 16(-3) = 52$. The pattern does not hold for $a_6$, so we calculate $a_7$: $a_7 = 4 - a_6(1 - a_5) = 4 - 52(1 - 16) = 4 - 52(-15) = 784$.

Next, we find $a_8$: $a_8 = 4 - a_7(1 - a_6) = 4 - 784(1 - 52) = 4 - 784(-51) = 39988$. Finally, we calculate $a_9$: $a_9 = 4 - a_8(1 - a_7) = 4 - 39988(1 - 784) = 4 - 39988(-783) = 31310608$.

Thus, $a_9 = 31310608$..&#x20;




___
The recurrence relation given is $a_n = 4 - a_{n-1} + a_{n-1} \cdot a_{n-2}$ for $n > 2$. Simplifying this, we can rewrite it as $a_n = 4 - a_{n-1}(1 - a_{n-2})$. Using the initial values $a_1 = 1$ and $a_2 = 1$, we calculate $a_3$ as follows: 
$$
\begin{align}
a_{3}&= 4 - a_{2}(1 - a_1) \\
&=  4 - 1(1 - 1) \\
&=  4
\end{align}
$$
Next, we find $a_4$: 
$$
\begin{align}
a_{4 }&= 4 - a_3(1 - a_2) \\
&= 4 - 4(1 - 1) \\
&= 4\\
\end{align}
$$
Observing that $a_3$ and $a_4$ are both 4, we proceed to calculate $a_5$: 
$$
\begin{align*}
a_{5} &=  4 - a_4(1 - a_3) \\
&=  4 - 4(1 - 4)  \\
&= 4 - 4(-3) \\
&=  16
\end{align*}
$$

Continuing, we calculate $a_6$:
$$
\begin{align*}
a_6 &= 4 - a_5(1 - a_4) \\
&=  4 - 16(1 - 4) \\
&=  4 - 16(-3) \\
&=  52
\end{align*}
$$
The pattern does not hold for $a_6$, so we calculate $a_7$: 
$$
\begin{align*}
a_7 &= 4 - a_6(1 - a_5) \\
&=  4 - 52(1 - 16) \\
&=  4 - 52(-15) \\
&=  784
\end{align*}
$$

Next, we find $a_8$:
$$
\begin{align*}
a_8 &= 4 - a_7(1 - a_6) \\
&=  4 - 784(1 - 52) \\
&=  4 - 784(-51) \\
&=  39988
\end{align*}
$$Finally, we calculate $a_9$:
$$
\begin{align*}
a_9 &= 4 - a_8(1 - a_7) \\
&=  4 - 39988(1 - 784) \\
&=  4 - 39988(-783) \\
&=  31310608
\end{align*}
$$

Thus, $a_9 = 31310608$.
