Given the quadratic equation:  
$\frac{2}{3}x^2 - 75x + 316 = 0$

The quadratic formula is:  
$x = \frac{-b \pm \sqrt{b^2 - 4ac}}{2a}$

Substitute a = \frac{2}{3}, b = -75, and c = 316 into the formula

$x = \frac{-(-75) \pm \sqrt{(-75)^2 - 4(-\frac{2}{3})(316)}}{2(\frac{2}{3})}$

Simplify step by step:

$-(-75) = 75$  
$(-75)^2 = 5625$  
$-4(-\frac{2}{3})(316) = -\frac{8}{3}(316) = -843.33$  
The discriminant becomes $5625 - 843.33 = 4778.67$  
$ 2(\frac{2}{3}) = \frac{4}{3} $.  
Thus, the formula becomes:  
$x = \frac{75 \pm \sqrt{4778.67}}{\frac{4}{3}}$

Multiply numerator and denominator by 3 to simplify:  
$x = \frac{225 \pm 3\sqrt{4778.67}}{4}$

So, the roots are:  
$x_1 = \frac{225 + \sqrt{19403}}{4}$  
$x_2 = \frac{225 - \sqrt{19403}}{4}$


I'll solve this step by step using the quadratic formula: The quadratic formula states that for an equation ax^2 + bx + c = 0, the roots are given by x = \frac{-b \pm \sqrt{b^2 - 4ac}}{2a}Here, a = 2/3, b = -75, and c = 316Let's substitute these values: x = \frac{-(-75) \pm \sqrt{(-75)^2 - 4(2/3)(316)}}{2(2/3)}x = \frac{75 \pm \sqrt{5625 - 4(2/3)(316)}}{4/3}x = \frac{75 \pm \sqrt{5625 - 4(2/3)(316)}}{4/3}x = \frac{75 \pm \sqrt{5625 - \frac{2528}{3}}}{4/3}x = \frac{75 \pm \sqrt{\frac{16875}{3} - \frac{2528}{3}}}{4/3}x = \frac{75 \pm \sqrt{\frac{14347}{3}}}{4/3}

Now simplify the denominator by multiplying numerator and denominator by 3:

x = \frac{75(3) \pm \sqrt{\frac{14347}{3}(3^2)}}{4}x = \frac{225 \pm \sqrt{43041}}{4}

Finally, split into the two roots:

x_1 = \frac{225 + \sqrt{43041}}{4}x_2 = \frac{225 - \sqrt{43041}}{4}