![[Pasted image 20241025082220.png|500]]

![[Pasted image 20241025082240.png|700]]
$$\begin{aligned}
Q&= \int_{0}^{d/2}\int_{0}^{2\pi }v(R)R \text{ d}\theta \text{ d}R\\
&= \int_{0}^{d/2}\int_{0}^{2\pi }v_{0}\left[1-\left(\frac{R}{d_{0}/2} \right)^{2} \right]R \text{ d}\theta \text{ d}R\\
&= 2\pi \int_{0}^{d/2}v_{0}R-\frac{R^{3}}{(d_{0}/2)^2}\text{ d}R\\
&= 2\pi \left[\frac{1}{2}v_{0}R^{2}- \frac{1}{4}\frac{R^{4}}{(d_{0}/2)^{2}} \right]_{0}^{d/2}\\
&= 2\pi \left(\frac{1}{2}v_{0}\frac{d_{0}}{4}-\frac{1}{4}\frac{(d_{0}/2)^{4}}{(d_{0}/2)^{2}} \right)\\
&= \frac{1}{4}\pi v_{0}d_{0}^{2}-\frac{1}{8}\pi d_{0}^{2}\\
&= \frac{1}{8}\pi v_{0}d_{0}^{2}
\end{aligned}$$
![[Pasted image 20241025083059.png|700]]
Constant $Q$ so
$$\begin{aligned}
\int_{0}^{d/2}\int_{0}^{2\pi }v_{1}\left[1-\left(\frac{R}{d_{1}/2} \right)^{2} \right]R \text{ d}\theta \text{ d}R&= \frac{1}{8}\pi v_{0}d_{0}^{2}\\
\frac{1}{8}\pi v_{1}d_{1}^{2}&= \frac{1}{8}v_{0}d_{0}^{2}\\
v_{1}&= \left(\frac{d_{0}}{d_{1}} \right)^{2}v_{0}\\
&= \left(\frac{2}{3} \right)^{2}\cdot 2\\
&= \frac{8}{9}
\end{aligned}$$
![[Pasted image 20241025083708.png|700]]
$$\begin{aligned}
p_{1}+\frac{1}{2}\rho v_{1}^{2}+\rho g h_{1}&= p_{0}+\frac{1}{2}\rho v_{0}^{2}+\rho g h_{0}\\
p_{1}&= p_{0}+\frac{1}{2}\rho  \left(v_{0}^{2}-v_{1}^{2} \right)+\rho g(h_{0}-h_{1})\\
p_{1}&= 16 \text{ kPa}+ \frac{1}{2}\cdot 1000 \,\mathrm{kg/m^{3}}\cdot \left(2^{2}\,\mathrm{m^{2}/s^{2}}-\left(\frac{8}{9}\right)^{2} \,\mathrm{m^{2}/s^{2}}\right)+ 1000 \,\mathrm{kg/m^{3}} \cdot 9.81 \,\mathrm{m/s^{2}} \cdot (1.5\text{ m}-0.7\cdot 1.5\text{ m})\\
&= 22019 \,\mathrm{Nm^{-2}}\\
&= 22 \text{ kPa}
\end{aligned}$$
![[Pasted image 20241025084506.png|700]]
Bernoulli simplification:
* Perfect fluid, $\mu =0$, but blood has some viscosity which gives resistance to flow$\quad\implies\quad$ pressure drop.
![[Pasted image 20241025084926.png|700]]
![[Pasted image 20241025084941.png|500]]
$$\begin{aligned}
(\tau _{y})^{1/3}&= 0.007(H-3.2)\\
&= 0.007(50-3.2)\\
&= 0.32\\
\tau _{y}&= 0.32^{3}\\
&= 0.035 \mathrm{\frac{dyne}{cm}}\\
&= 0.035 \cdot 10 ^{-4} \text{ kPa}\\
&= 3.5 \cdot 10^{-6}\text{ kPa}
\end{aligned}$$
![[Pasted image 20241025085547.png|700]]
Plug flow (Cassons model)
![[Pasted image 20241025085816.png|700]]
Linear viscous flow: $\tau =\mu \dot \gamma$. Put this into Cauchys equations to get Navier Stokes equation.
![[Pasted image 20241025091642.png|500]]
![[Pasted image 20241025091659.png|500]]
![[Pasted image 20241025091716.png|600]]
* Uncoiling of fibers in direction $\mathbf a_{02}$.

![[Pasted image 20241025092140.png|700]]
Incompressible$\quad\implies\quad \det F=1$. 
$$F=\begin{bmatrix}\lambda _{1}  \\  & \lambda _{2} \\  &   & \lambda _{3}\end{bmatrix}$$
Uniaxial testing in the 1-direction, then $\lambda _{2}=\lambda _{3}$ and for incompressibility: $\lambda _{1}\lambda _{2}\lambda _{3}=1$. Then $\lambda _{2}=\lambda _{3}= \frac{1}{\sqrt{\lambda _{1}}}$ and
$$F^{1}=\begin{bmatrix}\lambda _{1}  \\  & \frac{1}{\sqrt{\lambda _{1}}} \\  &   & \frac{1}{\sqrt{\lambda _{1}}}\end{bmatrix}$$
In the 2-direction:
$$F^{2}=\begin{bmatrix}\frac{1}{\sqrt{\lambda _{2}}}  \\  & \lambda _{2} \\  &   & \frac{1}{\sqrt{\lambda _{2}}}\end{bmatrix}$$
![[Pasted image 20241025092750.png|700]]
$$\Psi (I_{1},I_{4},J)=\frac{1}{2}\left[\mu (I_{1}-3)+\frac{k_{1}}{2k_{2}}(\exp(k_{2}(I_{4}-1)^{2})-1) \right]+p(J-1)$$
$$\begin{aligned}
S_{ij}&= 2 \left(\frac{\partial \Psi }{\partial I_{1}}\frac{\partial I_{1}}{\partial C_{ij}}
+\frac{\partial \Psi }{\partial I_{4}}\frac{\partial I_{4}}{\partial C_{ij}}
+ \frac{\partial \Psi }{\partial J}\frac{\partial J}{\partial C_{ij}} \right)\\
&= 2 \left(\frac{\mu }{2}\delta _{ij}+\frac{1}{2}k_{1}(I_{4}-1)\exp(k_{2}(I_{4}-1)^{2})  a_{0i}a_{0j}+p \frac{1}{2}JC_{ij}^{-1} \right)\\
&= \mu \delta _{ij}+k_{1}(I_{4}-1)\exp(k_{2}(I_{4}-1)^{2})a_{0i}a_{0j}+pJ C^{-1}_{ij}
\end{aligned}$$
$$\begin{aligned}
\sigma &= \frac{1}{J}FSF^{T}\\
&= \frac{1}{J} \left(\mu FF^{T}+ k_{1}(I_{4}-1)\exp(k_{2}(I_{4}-1)^{2})Fa \otimes aF^{T}+pJFC^{-1}_{ij}F^{T} \right)\\
&= \mu FF^{T}+ k_{1}(I_{4}-1)\exp(k_{2}(I_{4}-1)^{2})Fa_{0} \otimes a_{0}pF^{T}+pJF(F^{T}F)^{-1}F^{T} \\
&= \mu FF^{T}+ k_{1}(I_{4}-1)\exp(k_{2}(I_{4}-1)^{2})Fa_{0} \otimes a_{0}F^{T}+p I
\end{aligned}$$
For strip 1: $a_{0}=\begin{bmatrix}1 \\ 0\end{bmatrix}$ and $F^{1}=\begin{bmatrix}\lambda _{1}  \\  & \frac{1}{\sqrt{\lambda _{1}}} \\  &   & \frac{1}{\sqrt{\lambda _{1}}}\end{bmatrix}$ .
$$\begin{aligned}
\sigma ^{1}&= \mu \begin{bmatrix}\lambda _{1}^{2}\\
 & \frac{1}{\lambda_{1} }\\
 &   & \frac{1}{\lambda _{1}}\end{bmatrix}+k_{1}(I_{4}-1)\exp(k_{2}(I_{4}-1)^{2})\begin{bmatrix}\lambda _{1}\\
0\\
0\end{bmatrix}\otimes \begin{bmatrix}\lambda _{1}\\
0\\
0\end{bmatrix}+pI
\end{aligned}$$
So $\sigma _{2}=\sigma _{3}=0$, giving that
$$\begin{aligned}
\frac{\mu }{\lambda _{1}}+p&= 0\\
p&= -\frac{\mu }{\lambda _{1}}
\end{aligned}$$
Then,
$$\begin{aligned}
\sigma _{1}&= \mu \lambda _{1}^{2}+k_{1}(I_{4}-1)\exp(k_{2}(I_{4}-1)^{2})\lambda _{1}^{2}+p\\
&= (\mu +k_{1}(I_{4}-1)\exp(k_{2}(I_{4}-1)^{2}))\lambda _{1}^{2}-\frac{\mu }{\lambda _{1}}
\end{aligned}$$
Since $I_{4}=a_{0}Ca_{0}=a \cdot a$, 
$$I_{4}^{1}=\lambda _{1}^{2}$$
Finally,
$$\begin{aligned}
\sigma _{1}&= (\mu +k_{1}(\lambda _{1}^{2}-1)\exp(k_{2}(\lambda _{1}^{2}-1)^{2}))\lambda _{1}^{2}-\frac{\mu }{\lambda _{1}}
\end{aligned}$$

But! No collagen fibers in the 1-direction, so the exponential term is zero! Then
$$\begin{aligned}
\sigma _{1}&= \mu \lambda _{1}^{2}-\frac{\mu }{\lambda _{1}}
\end{aligned}$$

For strip 2:
$a_{0}=\begin{bmatrix}0  \\ 1\end{bmatrix}$ and $F^{2}=\begin{bmatrix}\frac{1}{\sqrt{\lambda _{2}}}  \\  & \lambda _{2} \\  &   & \frac{1}{\sqrt{\lambda _{2}}}\end{bmatrix}$. Then,
$$\begin{aligned}
\sigma ^{2}&= \mu \begin{bmatrix}\frac{1}{\lambda _{2}}  \\  & \lambda _{2}^{2} \\  &   & \frac{1}{\lambda _{2}}\end{bmatrix}
 +k_{1}(I_{4}-1)\exp(k_{2}(I_{4}-1)^{2})\begin{bmatrix}0\\
\lambda _{2}\\
0\end{bmatrix}\otimes \begin{bmatrix}0\\
\lambda _{2}\\
0\end{bmatrix}+pI
\end{aligned}$$
$$\begin{aligned}
\sigma _{3}&= \frac{\mu }{\lambda _{2}}+p=0\\
p&= -\frac{\mu }{\lambda _{2}}
\end{aligned}$$
Finally, with $I_{4}=\lambda _{2}^{2}$
$$\begin{aligned}
\sigma _{2}&= \mu \lambda _{2}^{2}+k_{1}(\lambda _{2}^{2}-1)\exp(k_{2}(\lambda _{2}^{2}-1)^{2})-\frac{\mu }{\lambda _{2}}
\end{aligned}$$