
## Notes
![[Pasted image 20231016114240.png|700]]





![[Pasted image 20231016113810.png|800]]

![[Pasted image 20231016113822.png|800]]
$$\Bigg\{\begin{align*}
(\partial _{t}-\Delta  )G(t,x,s,y)  &=\delta _{0}((t,x)-(s,y)) \quad&\text{in }\mathbb{R}_{t}\times(0,\infty )_{x} \\
G(t,x,s,y)  &=0 \quad&\text{on }\mathbb{R}_{t}\times \{0,\infty \}_{x}\\
G(t,x,s,y)  &=0 \quad&\text{in }(t,x)\in (-\infty,s)\times(0,\infty)_{x}
\end{align*}$$
If we set $G(t,x,s,y)=E_{+}(t-s,x-y)- E_{+}(t-s,y)= \mathbb 1_{(0,\infty)}(t-s) \frac{1}{(4\pi (t-s))^{\frac{d}{2}}}e^{- \frac{\lvert x-y \rvert^{2}}{4(t-s)}}-\mathbb 1_{(0,\infty)}(t-s) \frac{1}{(4\pi (t-s))^{\frac{d}{2}}}e^{- \frac{\lvert y \rvert^{2}}{4(t-s)}}$,
the third equation is solved. Further, both for $x=0$ and $x\to\infty$, we have that $G(t,0,s,y)=0$

$$G(t,x,s,y)=E_{+}(t-s,x-y)$$

![[Pasted image 20231016113832.png|800]]

![[Pasted image 20231016113841.png|800]]