Alexander Hatle

![[Pasted image 20231112170327.png]]
![[Pasted image 20231112170954.png]]
I will denote $h=\frac{1}{N+1}$.
Using the trig identities
$$\begin{align*}
\text{sin}(A-B)&= \text{sin}A \text{cos}B-\text{cos}A \text{sin}B,\\
\text{sin}(A+B)&= \text{sin}A \text{cos}B+\text{cos}A \text{sin}B,
\end{align*}$$
we can simply verify that
$$\begin{align*}
(T_{N}z_{j})(k)&=  \sqrt{2h}\left(2\text{sin}\left(j \pi k h \right)-\text{sin}(j\pi (k-1)h)-\text{sin}(j\pi (k+1)h) \right)\\
&= \sqrt{2h}(2\text{sin}(j \pi k h)- \text{sin}(j \pi kh)\text{cos}(j\pi  h)+\text{cos}(j \pi k h)\text{sin}(j\pi  h)-\text{sin}(j \pi k h)\text{cos}(j\pi  h)+\text{cos}(j \pi k h)\text{sin}(j\pi h))\\
&= \sqrt{2h}\cdot \text{sin}(j \pi kh)2(1-\text{cos}(j\pi h))\\
&= 2(1-\text{cos}(j \pi h))z_{j}(k).
\end{align*}$$
There are $N$ nonzero eigenvectors $z_{j}(k)$, $j=1,\dots ,N$. As we already have $N$ eigenvectors, there are no other eigenvectors.

<div style="page-break-after: always;"></div>

![[Pasted image 20231115181711.png|800]]
![[Pasted image 20231115181632.png|800]]
![[Pasted image 20231115181619.png|800]]
We can write
$$\begin{align*}
	XB(i,j)&= \sum_{k}^{}X_{ik}B_{kj}
\\
XB(:,j)&= \begin{bmatrix}\sum_{k} X_{1k}B_{kj} \\ \vdots  \\ \sum_{k} X_{nk}B_{kj}\end{bmatrix}\\
	&= \sum_{k}^{}\begin{bmatrix}X_{1k}\\
\vdots \\
X_{nk}\end{bmatrix} B_{kj}\\
&= \sum_{k}^{}X(:,k)B_{kj}
\end{align*}$$
While the LHS is
$$\begin{align*}
(B^{T}\otimes I_{m})\cdot \text{vec}(X)&= \begin{bmatrix}B_{11}I_{m} & \dots  & B_{n1}I_{m} \\ \vdots  & \ddots  & \vdots  \\ B_{1n}I_{m} & \dots  & B_{nn}I_{m}\end{bmatrix}\begin{bmatrix}X(:,1 ) \\ \vdots   \\ X(:,n) \end{bmatrix}\\
&= \begin{bmatrix}B_{11}X(:,1)+\dots +B_{n1}X(:,n)\\
\vdots \\
B_{1n}X(:,1)+\dots +B_{nn}X(:,n)\end{bmatrix}\\
&= \begin{bmatrix}\sum_{k}^{}X(:,k)B_{k1}\\
\vdots \\
\sum_{k}^{}X(:,k)B_{kn}\end{bmatrix}\\
&= \begin{bmatrix}XB(:,1)\\
\vdots \\
XB(:,n)\end{bmatrix}\\
&= \text{vec}(XB)
\end{align*}$$

![[Pasted image 20231115181729.png|800]]
![[Pasted image 20231112171638.png]]
$$\begin{align*}
(A \otimes B)\cdot (C \otimes D)&= \begin{bmatrix}A_{11}B & \dots  & A_{1n}B \\ \vdots  & \ddots  & \vdots  \\ A_{n1}B & \dots  & A_{nn}B\end{bmatrix}\cdot 
\begin{bmatrix}C_{11}D & \dots  & C_{1n}D \\ \vdots  & \ddots  & \vdots  \\ C_{n1}D & \dots  & C_{nn}D\end{bmatrix}\\
((A \otimes B)\cdot (C \otimes D))_{ij}&= \sum_{k}^{}A_{ik}B \cdot C_{kj}D\\
&= \sum_{k}^{}A_{ik}C_{kj}\cdot BD\\
&= (AC)_{ij}\cdot BD\\
&= ((AC)\otimes (BD) )_{ij}\\
(A \otimes B)\cdot (C \otimes D)&= (AC)\otimes (BD)
\end{align*}$$

![[Pasted image 20231112171646.png]]

$$\begin{align*}
((A^{-1}\otimes B^{-1}) (A \otimes B))_{ij}&= \sum_{k}^{}(A^{-1})_{ik}B^{-1} A_{kj}B\\
&= \sum_{k}^{}(A^{-1})_{ik}A_{kj}\\
&= (A^{-1}A)_{ij}\\
(A^{-1}\otimes B^{-1}) (A \otimes B)&= I
\end{align*}$$
$$\begin{align*}
((A \otimes B)(A^{-1} \otimes B^{-1}))_{ij}&= \sum_{k}^{}A_{ik}B(A^{-1})_{kj}B^{-1}\\
&= (AA^{-1})_{ij}\\
(A \otimes B)(A^{-1} \otimes B^{-1})&= I
\end{align*}$$
Since $(A^{-1}\otimes B^{-1})$ is both a right and left inverse, 
$$(A \otimes B)^{-1}=(A^{-1}\otimes B^{-1})$$

For the transpose
$$\begin{align*}
(A \otimes B)^{T}&= \begin{bmatrix}A_{11}B & \dots &  A_{1n}B\\
\vdots  & \ddots  & \vdots \\
A_{n1}B & \dots  &  A_{nn}B \end{bmatrix}^{T}\\
&= \begin{bmatrix}A_{11}B^{T} & \dots &  A_{n1}B^{T}\\
\vdots  & \ddots  & \vdots \\
A_{1n}B^{T} & \dots  &  A_{nn}B^{T} \end{bmatrix}\\
&= A^{T}\otimes B^{T}
\end{align*}$$
![[Pasted image 20231115182116.png|800]]
![[Pasted image 20231115181810.png|800]]
$$\begin{align*}
AX+XB&= C\\
\text{vec}(AX+XB)&= \text{vec}(C)
\end{align*}$$
Using Lemma 6.2.1 and 6.2.2, we get that the Sylvester equation is equivalent to
$$\begin{align*}
(I_{m}\otimes A)\cdot \text{vec}(X)+(B^{T} \otimes I_{n})\cdot \text{vec}(X)&= \text{vec}(C)\\
(I_{m}\otimes A+B^{T} \otimes I_{n})\cdot \text{vec}(X)&= \text{vec}(C).
\end{align*}$$
![[Pasted image 20231115181845.png|800]]
Lemma 6.2 says that 
$$\begin{align*}
	\text{vec}(AX)&= (I_{n}\otimes A )\cdot \text{vec}X\\
\text{vec}(XB)&= (B^{T}\otimes I_{m})\cdot \text{vec}X
\end{align*}$$
Then,
$$\begin{align*}
\text{vec}(A(XB))&= (I\otimes A)\cdot \text{vec}(XB)\\
&= (I\otimes A)\cdot (B^{T}\otimes I) \cdot \text{vec}X\\
&= (I \cdot B^{T})\otimes (A \cdot I) \cdot \text{vec}X\\
\text{vec}(AXB)&= (B^{T}\otimes A)\cdot \text{vec}X
\end{align*}$$
<div style="page-break-after: always;"></div>

![[Pasted image 20231112170722.png]]
- Page 357, Question 6.5, Part 1: The expression for the eigenvectors should be: "z_ij, where z_ij = kron(y_j, x_i) whose ((l-1)\*m+k)th entry is x_i(k)\*y_j(l)" {using Matlab notation kron() for the Kronecker product}

Using lemma 6.3.1,
$$\begin{align*}
(I_{m}\otimes A+B \otimes I_{n})(Y \otimes X)&= (I_{m}\otimes A)(Y \otimes X)+(B \otimes I_{n})(Y \otimes X)\\
&= (I_{m}\cdot Y)\otimes (A \cdot X)+ (B \cdot Y)\otimes (I_{n}\cdot X)\\
&= (I_{m}\cdot Y)\otimes (X \cdot \Lambda _{A})+ (Y \cdot \Lambda _{B})\otimes (I_{n}\cdot X)\\
&= (Y \cdot I_{m})\otimes (X \cdot \Lambda _{A})+ (Y \cdot \Lambda _{B})\otimes ( X \cdot I_{n})\\
&= (Y \otimes X)\cdot (I_{m}\otimes \Lambda _{A})+(Y \otimes X)\cdot (\Lambda _{B} \otimes I_{n})\\
&= (Y \otimes X)\cdot (I_{m}\otimes \Lambda _{A}+\Lambda _{B}\otimes I_{n})
\end{align*}$$
where in line 5, I have used lemma 6.3.1 in reverse.

![[Pasted image 20231112170729.png]]
(I assume that it should say $\alpha _{i}+\beta _{j}≠0$)
In question 6.4.3 we showed that the Sylvester equation $AX+XB^{T}=C$ is equivalent to 
$$(I_{m}\otimes A+B \otimes I_{n})\cdot \text{vec}(X)= \text{vec}(C).$$

The Sylvester equation is nonsingular if and only if $I_{m}\otimes A+B \otimes I_{n}$ is nonsingular if and only if all its eigenvalues are nonzero.
In the last question, we showed that we can write the eigenvalues of $I_{m}\otimes A+B \otimes I_{n}$ as $\lambda _{ij}=\alpha _{i}+\beta _{j}$.

Thus, the Sylvester equation $AX+XB^{T}=C$ is nonsingular if and only if $\alpha _{i}+\beta _{j}≠0$ for all eigenvalues $\alpha _{i}$ of $A$ and $\beta _{j}$ of $B$.

The same is true for $AX+XB^{T}=C$ since $B$ and $B^{T}$ share eigenvalues.
![[Pasted image 20231112170735.png]]
- Page 358, Question 6.5, Part 3: "(km+l)th entry" should be "((k-1)\*m+l)th" entry.
- Page 358, Question 6.5, Part 3: Equation (6.64) should be "(A kron B)(X kron Y) = (X kron Y)(Lambda_A kron Lambda_B)", although (6.64) is also mathematically correct. (Mathias Weiden)

We want to show that
$$(A \otimes B)\cdot (X \otimes Y)=(X \otimes Y)\cdot (\Lambda _{A}\otimes \Lambda _{B})$$
Using lemma 6.3.1, we can write the LHS as
$$\begin{align*}
(A \otimes B)\cdot (X \otimes  Y)&= (A \cdot X)\otimes (B \cdot Y)\\
&= (X \cdot \Lambda _{A})\otimes (Y \cdot \Lambda _{B})\\
&= (X \otimes Y) \cdot (\Lambda _{A}\otimes \Lambda _{B}),
\end{align*}$$
which is what we wanted to show.