![[Pasted image 20231206133057.png|800]]


![[Pasted image 20231206133230.png|800]]
![[Pasted image 20231206133243.png|800]]
![[Pasted image 20231206133132.png|800]]
Starting with $\hat p_{1}=\hat b = M^{-1/2}b$, we can get that 
$$\hat z= \hat A \cdot \hat p_{k}\stackrel{\text{for }k=1}{=}M^{-1/2}AM^{1/2}M^{-1/2}b=M^{-1/2}z$$
$$\begin{align*}
\hat \nu _{k}&= \frac{\hat r_{k-1}^{T}\hat r_{k-1}}{\hat p_{k}^{T}\hat z}\\
&= \frac{\hat r_{k-1}^{T}\hat r_{k-1}}{\hat p_{k}^{T}\hat A \hat p_{k}}
\end{align*}$$

$$\hat r_{k}=\hat r_{k-1} -\hat \nu _{k}\hat p_{k}$$







