Alexander Hatle

![[Pasted image 20240411150753.png]]
$$\begin{align*}
L&= \pi ^{2} + \lambda (u^{n}-\overline{u}-(\pi -\pi ^{e}))^{2}\\
\frac{\text{d}L}{\text{d}\pi }&= 2\pi^{*} -2\lambda (u^{n}-\overline{u}-(\pi^{*} -\pi ^{e}))=0
\end{align*}$$
assuming that $\pi ^{*}=\pi ^{e}$,
$$\begin{align*}
\pi ^{*}&= \lambda (u^{n}-\overline{u})\\
&= 2 \cdot 2=4
\end{align*}$$

![[Pasted image 20240411151434.png]]
$$\begin{align*}
\pi ^{*}&= \lambda (u^{n}-\overline{u})\\
&= 100 \cdot 2=200
\end{align*}$$

![[Pasted image 20240411152405.png]]